driver/Clflags.ml
@@ -22,6 +22,7 @@ let option_fbitfields = ref false
 let option_fvararg_calls = ref true
 let option_fpacked_structs = ref false
 let option_fmadd = ref false
+let option_fsse = ref true
 let option_dparse = ref false
 let option_dcmedium = ref false
 let option_dclight = ref false
