driver/Interp.ml
@@ -1,0 +1,408 @@
+(* *********************************************************************)
+(*                                                                     *)
+(*              The Compcert verified compiler                         *)
+(*                                                                     *)
+(*          Xavier Leroy, INRIA Paris-Rocquencourt                     *)
+(*                                                                     *)
+(*  Copyright Institut National de Recherche en Informatique et en     *)
+(*  Automatique.  All rights reserved.  This file is distributed       *)
+(*  under the terms of the INRIA Non-Commercial License Agreement.     *)
+(*                                                                     *)
+(* *********************************************************************)
+
+(* Interpreting CompCert C sources *)
+
+open Format
+open Camlcoq
+open Datatypes
+open BinPos
+open BinInt
+open AST
+open Values
+open Memory
+open Globalenvs
+open Events
+open Csyntax
+open Csem
+open Clflags
+
+(* Configuration *)
+
+let trace = ref 1   (* 0 if quiet, 1 if normally verbose, 2 if full trace *)
+
+type mode = First | Random | All
+
+let mode = ref First
+
+(* Printing events *)
+
+let print_eventval p = function
+  | EVint n -> fprintf p "%ld" (camlint_of_coqint n)
+  | EVfloat f -> fprintf p "%F" f
+  | EVptr_global(id, ofs) -> 
+      fprintf p "&%s%+ld" (extern_atom id) (camlint_of_coqint ofs)
+
+let print_eventval_list p = function
+  | [] -> ()
+  | v1 :: vl ->
+      print_eventval p v1;
+      List.iter (fun v -> fprintf p ",@ %a" print_eventval v) vl
+
+let print_event p = function
+  | Event_syscall(id, args, res) ->
+      fprintf p "extcall %s(%a) -> %a"
+                (extern_atom id)
+                print_eventval_list args
+                print_eventval res
+  | Event_vload(chunk, id, ofs, res) ->
+      fprintf p "volatile load %s[&%s%+ld] -> %a"
+                (PrintCminor.name_of_chunk chunk)
+                (extern_atom id) (camlint_of_coqint ofs)
+                print_eventval res
+  | Event_vstore(chunk, id, ofs, arg) ->
+      fprintf p "volatile store %s[&%s%+ld] <- %a"
+                (PrintCminor.name_of_chunk chunk)
+                (extern_atom id) (camlint_of_coqint ofs)
+                print_eventval arg
+  | Event_annot(text, args) ->
+      fprintf p "annotation \"%s\" %a"
+                (extern_atom text)
+                print_eventval_list args
+
+(* Printing states *)
+
+let name_of_fundef prog fd =
+  let rec find_name = function
+  | [] -> "<unknown function>"
+  | Coq_pair(id, fd') :: rem ->
+      if fd = fd' then extern_atom id else find_name rem
+  in find_name prog.prog_funct
+
+let name_of_function prog fn =
+  name_of_fundef prog (Internal fn)
+
+let print_val p = function
+  | Vint n -> fprintf p "%ld" (camlint_of_coqint n)
+  | Vfloat f -> fprintf p "%F" f
+  | Vptr(b, ofs) -> fprintf p "<ptr>"
+  | Vundef -> fprintf p "<undef>"
+
+let print_val_list p = function
+  | [] -> ()
+  | v1 :: vl ->
+      print_val p v1;
+      List.iter (fun v -> fprintf p ",@ %a" print_val v) vl
+
+let print_state prog p = function
+  | State(f, s, k, e, m) ->
+      fprintf p "in function %s, statement@ @[<hv 0>%a@]"
+              (name_of_function prog f)
+              PrintCsyntax.print_stmt s 
+  | ExprState(f, r, k, e, m) ->
+      fprintf p "in function %s, expression@ @[<hv 0>%a@]"
+              (name_of_function prog f)
+              PrintCsyntax.print_expr r
+  | Callstate(fd, args, k, m) ->
+      fprintf p "calling@ @[<hov 2>%s(%a)@]"
+              (name_of_fundef prog fd)
+              print_val_list args
+  | Returnstate(res, k, m) ->
+      fprintf p "returning@ %a"
+              print_val res
+
+let mem_of_state = function
+  | State(f, s, k, e, m) -> m
+  | ExprState(f, r, k, e, m) -> m
+  | Callstate(fd, args, k, m) -> m
+  | Returnstate(res, k, m) -> m
+
+(* Comparing memory states *)
+
+let rec compare_Z_range lo hi f =
+  if coq_Zcompare lo hi = Lt then begin
+    let c = f lo in if c <> 0 then c else compare_Z_range (coq_Zsucc lo) hi f
+  end else 0
+
+let compare_mem m1 m2 =
+  if m1 == m2 then 0 else
+  let c = compare m1.Mem.nextblock m2.Mem.nextblock in if c <> 0 then c else
+  compare_Z_range Z0 m1.Mem.nextblock (fun b ->
+    let (Coq_pair(lo, hi) as bnds) = m1.Mem.bounds b in
+    let c = compare bnds (m2.Mem.bounds b) in if c <> 0 then c else
+    let contents1 = m1.Mem.mem_contents b and contents2 = m2.Mem.mem_contents b in
+    if contents1 == contents2 then 0 else
+    let c = compare_Z_range lo hi (fun ofs ->
+               compare (contents1 ofs) (contents2 ofs)) in if c <> 0 then c else
+    let access1 = m1.Mem.mem_access b and access2 = m2.Mem.mem_access b in
+    if access1 == access2 then 0 else
+    compare_Z_range lo hi (fun ofs -> compare (access1 ofs) (access2 ofs)))
+
+(* Comparing continuations *)
+
+let some_expr = Evar(Coq_xH, Tvoid)
+
+let rank_cont = function
+  | Kstop -> 0
+  | Kdo _ -> 1
+  | Kseq _ -> 2
+  | Kifthenelse _ -> 3
+  | Kwhile1 _ -> 4
+  | Kwhile2 _ -> 5
+  | Kdowhile1 _ -> 6
+  | Kdowhile2 _ -> 7
+  | Kfor2 _ -> 8
+  | Kfor3 _ -> 9
+  | Kfor4 _ -> 10
+  | Kswitch1 _ -> 11
+  | Kswitch2 _ -> 12
+  | Kreturn _ -> 13
+  | Kcall _ -> 14
+
+let rec compare_cont k1 k2 =
+  if k1 == k2 then 0 else
+  match k1, k2 with
+  | Kstop, Kstop -> 0
+  | Kdo k1, Kdo k2 -> compare_cont k1 k2
+  | Kseq(s1, k1), Kseq(s2, k2) ->  
+      let c = compare s1 s2 in if c <> 0 then c else compare_cont k1 k2
+  | Kifthenelse(s1, s1', k1), Kifthenelse(s2, s2', k2) ->
+      let c = compare (s1,s1') (s2,s2') in
+      if c <> 0 then c else compare_cont k1 k2
+  | Kwhile1(e1, s1, k1), Kwhile1(e2, s2, k2) ->
+      let c = compare (e1,s1) (e2,s2) in
+      if c <> 0 then c else compare_cont k1 k2
+  | Kwhile2(e1, s1, k1), Kwhile2(e2, s2, k2) ->
+      let c = compare (e1,s1) (e2,s2) in
+      if c <> 0 then c else compare_cont k1 k2
+  | Kdowhile1(e1, s1, k1), Kdowhile1(e2, s2, k2) ->
+      let c = compare (e1,s1) (e2,s2) in
+      if c <> 0 then c else compare_cont k1 k2
+  | Kdowhile2(e1, s1, k1), Kdowhile2(e2, s2, k2) ->
+      let c = compare (e1,s1) (e2,s2) in
+      if c <> 0 then c else compare_cont k1 k2
+  | Kfor2(e1, s1, s1', k1), Kfor2(e2, s2, s2', k2) ->
+      let c = compare (e1,s1,s1') (e2,s2,s2') in
+      if c <> 0 then c else compare_cont k1 k2
+  | Kfor3(e1, s1, s1', k1), Kfor3(e2, s2, s2', k2) ->
+      let c = compare (e1,s1,s1') (e2,s2,s2') in
+      if c <> 0 then c else compare_cont k1 k2
+  | Kfor4(e1, s1, s1', k1), Kfor4(e2, s2, s2', k2) ->
+      let c = compare (e1,s1,s1') (e2,s2,s2') in
+      if c <> 0 then c else compare_cont k1 k2
+  | Kswitch1(sl1, k1), Kswitch1(sl2, k2) ->
+      let c = compare sl1 sl2 in
+      if c <> 0 then c else compare_cont k1 k2
+  | Kreturn k1, Kreturn k2 ->
+      compare_cont k1 k2
+  | Kcall(f1, e1, c1, ty1, k1), Kcall(f2, e2, c2, ty2, k2) ->
+      let c = compare (f1, e1, c1 some_expr, ty1) (f2, e2, c2 some_expr, ty2) in
+      if c <> 0 then c else compare_cont k1 k2
+  | _, _ ->
+      compare (rank_cont k1) (rank_cont k2)
+
+(* Comparing states *)
+
+let rank_state = function
+  | State _ -> 0
+  | ExprState _ -> 1
+  | Callstate _ -> 2
+  | Returnstate _ -> 3
+
+let compare_state s1 s2 =
+  if s1 == s2 then 0 else
+  match s1, s2 with
+  | State(f1,s1,k1,e1,m1), State(f2,s2,k2,e2,m2) ->
+      let c = compare (f1,s1,e1) (f2,s2,e2) in if c <> 0 then c else
+      let c = compare_cont k1 k2 in if c <> 0 then c else
+      compare_mem m1 m2
+  | ExprState(f1,r1,k1,e1,m1), ExprState(f2,r2,k2,e2,m2) ->
+      let c = compare (f1,r1,e1) (f2,r2,e2) in if c <> 0 then c else
+      let c = compare_cont k1 k2 in if c <> 0 then c else
+      compare_mem m1 m2
+  | Callstate(fd1,args1,k1,m1), Callstate(fd2,args2,k2,m2) ->
+      let c = compare (fd1,args1) (fd2,args2) in if c <> 0 then c else
+      let c = compare_cont k1 k2 in if c <> 0 then c else
+      compare_mem m1 m2
+  | Returnstate(res1,k1,m1), Returnstate(res2,k2,m2) ->
+      let c = compare res1 res2 in if c <> 0 then c else
+      let c = compare_cont k1 k2 in if c <> 0 then c else
+      compare_mem m1 m2
+  | _, _ ->
+      compare (rank_state s1) (rank_state s2)
+
+module StateSet =
+  Set.Make(struct type t = state let compare = compare_state end)
+
+(* Extract a string from a global pointer *)
+
+let extract_string ge m id ofs =
+  let b = Buffer.create 80 in
+  let rec extract blk ofs =
+    match Memory.Mem.load Mint8unsigned m blk ofs with
+    | Some(Vint n) ->
+        let c = Char.chr (Int32.to_int (camlint_of_coqint n)) in
+        if c = '\000' then begin
+          Some(Buffer.contents b)
+        end else begin
+          Buffer.add_char b c; 
+          extract blk (coq_Zsucc ofs)
+        end
+    | _ ->
+        None in
+  match Genv.find_symbol ge id with
+  | None -> None
+  | Some blk -> extract blk ofs
+
+(* Emulation of printf *)
+
+(* All ISO C 99 formats except size modifiers [ll] (long long) and [L]
+   (long double) *)
+
+let re_conversion = Str.regexp
+  "%[-+0# ]*[0-9]*\\(\\.[0-9]*\\)?\\([lhjzt]\\|hh\\)?\\([aAcdeEfgGinopsuxX%]\\)"
+
+external format_float: string -> float -> string
+  = "caml_format_float"
+external format_int32: string -> int32 -> string
+  = "caml_int32_format"
+
+let do_printf ge m fmt args =
+
+  let b = Buffer.create 80 in
+  let len = String.length fmt in
+
+  let opt_search_forward pos =
+    try Some(Str.search_forward re_conversion fmt pos)
+    with Not_found -> None in
+
+  let rec scan pos args =
+    if pos < len then begin
+    match opt_search_forward pos with
+    | None ->
+        Buffer.add_substring b fmt pos (len - pos)
+    | Some pos1 ->
+        Buffer.add_substring b fmt pos (pos1 - pos);
+        let pat = Str.matched_string fmt
+        and conv = Str.matched_group 3 fmt
+        and pos' = Str.match_end() in
+        match args, conv.[0] with
+        | _, '%' ->
+            Buffer.add_char b '%';
+            scan pos' args
+        | [], _ ->
+            Buffer.add_string b "<missing argument>";
+            scan pos' []
+        | EVint i :: args', ('d'|'i'|'u'|'o'|'x'|'X'|'c') ->
+            Buffer.add_string b (format_int32 pat (camlint_of_coqint i));
+            scan pos' args'
+        | EVfloat f :: args', ('f'|'e'|'E'|'g'|'G'|'a') ->
+            Buffer.add_string b (format_float pat f);
+            scan pos' args'
+        | EVptr_global(id, ofs) :: args', 's' ->
+            Buffer.add_string b
+              (match extract_string ge m id ofs with
+               | Some s -> s
+               | None -> "<bad string>");
+            scan pos' args'
+        | EVptr_global(id, ofs) :: args', 'p' ->
+            Printf.bprintf b "<&%s%+ld>" (extern_atom id) (camlint_of_coqint ofs);
+            scan pos' args'
+        | _ :: args', _ ->
+            Buffer.add_string b "<formatting error>";
+            scan pos' args'
+    end
+  in scan 0 args; Buffer.contents b
+
+(* Implementing external functions *)
+
+let re_stub = Str.regexp "\\$[if]*$"
+
+let chop_stub name = Str.replace_first re_stub "" name
+
+let rec world = Determinism.World(world_io, world_vload, world_vstore)
+
+and world_io id args =
+  match chop_stub(extern_atom id), args with
+  | "printf", EVptr_global(id, ofs) :: args' ->
+      Some(Coq_pair(EVint Integers.Int.zero, world))
+  | _, _ ->
+      None
+
+and world_vload chunk id ofs =
+  let res = match chunk with
+    | Mint8signed -> EVint(coqint_of_camlint(Int32.sub (Random.int32 0x100l) 0x80l))
+    | Mint8unsigned -> EVint(coqint_of_camlint(Random.int32 0x100l))
+    | Mint16signed -> EVint(coqint_of_camlint(Int32.sub (Random.int32 0x10000l) 0x8000l))
+    | Mint16unsigned -> EVint(coqint_of_camlint(Random.int32 0x10000l))
+    | Mint32 -> EVint(coqint_of_camlint(Random.int32 0x7FFF_FFFFl))
+    | Mfloat32 -> EVfloat(Floats.Float.singleoffloat(Random.float 1.0))
+    | Mfloat64 -> EVfloat(Random.float 1.0)
+  in Some(Coq_pair(res, world))
+
+and world_vstore chunk id ofs arg =
+  Some world
+
+let do_event p ge time s ev =
+  if !trace >= 1 then
+    fprintf p "@[<hov 2>Time %d: observable event: %a@]@."
+              time print_event ev;
+  match ev with
+  | Event_syscall(name, EVptr_global(id, ofs) :: args', res) 
+    when chop_stub (extern_atom name) = "printf" ->
+      flush stderr;
+      let m = mem_of_state s in
+      begin match extract_string ge m id ofs with
+      | Some fmt -> print_string (do_printf ge m fmt args')
+      | None -> print_string "<bad printf>\n"
+      end;
+      flush stdout
+  | _ -> ()
+
+let do_events p ge time s t =
+  List.iter (do_event p ge time s) t
+
+(* Exploration *)
+
+let do_step p prog ge time s =
+  if !trace >= 2 then
+    fprintf p "@[<hov 2>Time %d: %a@]@." time (print_state prog) s;
+  match Cexec.at_final_state s with
+  | Some r ->
+      if !trace >= 1 then begin
+        fprintf p "Time %d: program terminated (exit code = %ld)@."
+                  time (camlint_of_coqint r);
+        []
+      end else begin
+        exit (Int32.to_int (camlint_of_coqint r))
+      end
+  | None ->
+      match Cexec.do_step ge world s with
+      | [] ->
+          if !trace = 1 then
+            fprintf p "@[<hov 2>Time %d: %a@]@." time (print_state prog) s;
+          fprintf p "ERROR: Undefined behavior@.";
+          fprintf p "@].";
+          exit 126
+      | l ->
+          List.iter (fun (Coq_pair(t, s')) -> do_events p ge time s t) l;
+          List.map snd l
+
+let rec explore p prog ge time ss =
+  let succs =
+    StateSet.fold (fun s l -> do_step p prog ge time s @ l) ss [] in
+  if succs <> [] then begin
+    let ss' =
+      match !mode with
+      | First -> StateSet.singleton (List.hd succs)
+      | Random -> StateSet.singleton (List.nth succs (Random.int (List.length succs)))
+      | All -> List.fold_right StateSet.add succs StateSet.empty in
+    explore p prog ge (time + 1) ss'
+  end
+
+let execute prog =
+  let p = err_formatter in
+  pp_set_max_boxes p 10;
+  begin match Cexec.do_initial_state prog with
+  | None -> fprintf p "ERROR: Initial state undefined@."
+  | Some(Coq_pair(ge, s)) -> explore p prog ge 0 (StateSet.singleton s)
+  end
