cfrontend/Cexec.v
@@ -1,0 +1,1814 @@
+Require Import Axioms.
+Require Import Coqlib.
+Require Import Errors.
+Require Import Maps.
+Require Import Integers.
+Require Import Floats.
+Require Import Values.
+Require Import AST.
+Require Import Memory.
+Require Import Events.
+Require Import Globalenvs.
+Require Import Determinism.
+Require Import Csyntax.
+Require Import Csem.
+Require Cstrategy.
+
+(** Animating the CompCert C semantics *)
+
+Lemma type_eq: forall (ty1 ty2: type), {ty1=ty2} + {ty1<>ty2}
+with typelist_eq: forall (tyl1 tyl2: typelist), {tyl1=tyl2} + {tyl1<>tyl2}
+with fieldlist_eq: forall (fld1 fld2: fieldlist), {fld1=fld2} + {fld1<>fld2}.
+Proof.
+  assert (forall (x y: intsize), {x=y} + {x<>y}). decide equality.
+  assert (forall (x y: signedness), {x=y} + {x<>y}). decide equality.
+  assert (forall (x y: floatsize), {x=y} + {x<>y}). decide equality.
+  generalize ident_eq zeq. intros E1 E2. 
+  decide equality.
+  decide equality.
+  generalize ident_eq. intros E1.
+  decide equality.
+Defined.
+
+Opaque type_eq.
+
+(** Error monad with options or lists *)
+
+Notation "'do' X <- A ; B" := (match A with Some X => B | None => None end)
+  (at level 200, X ident, A at level 100, B at level 200)
+  : option_monad_scope.
+
+Notation " 'check' A ; B" := (if A then B else None)
+  (at level 200, A at level 100, B at level 200)
+  : option_monad_scope.
+
+Notation "'do' X <- A ; B" := (match A with Some X => B | None => nil end)
+  (at level 200, X ident, A at level 100, B at level 200)
+  : list_monad_scope.
+
+Notation " 'check' A ; B" := (if A then B else nil)
+  (at level 200, A at level 100, B at level 200)
+  : list_monad_scope.
+
+Definition is_val (a: expr) : option (val * type) :=
+  match a with
+  | Eval v ty => Some(v, ty)
+  | _ => None
+  end.
+
+Lemma is_val_inv:
+  forall a v ty, is_val a = Some(v, ty) -> a = Eval v ty.
+Proof.
+  intros until ty. destruct a; simpl; congruence.
+Qed.
+
+Definition is_loc (a: expr) : option (block * int * type) :=
+  match a with
+  | Eloc b ofs ty => Some(b, ofs, ty)
+  | _ => None
+  end.
+
+Lemma is_loc_inv:
+  forall a b ofs ty, is_loc a = Some(b, ofs, ty) -> a = Eloc b ofs ty.
+Proof.
+  intros until ty. destruct a; simpl; congruence.
+Qed.
+
+Local Open Scope option_monad_scope. 
+
+Fixpoint is_val_list (al: exprlist) : option (list (val * type)) :=
+  match al with
+  | Enil => Some nil
+  | Econs a1 al => do vt1 <- is_val a1; do vtl <- is_val_list al; Some(vt1::vtl)
+  end.
+
+Definition is_skip (s: statement) : {s = Sskip} + {s <> Sskip}.
+Proof.
+  destruct s; (left; congruence) || (right; congruence).
+Qed.
+
+(** * Reduction of expressions *)
+
+Section EXEC.
+
+Variable ge: genv.
+
+Inductive reduction: Type :=
+  | Lred (l': expr) (m': mem)
+  | Rred (r': expr) (m': mem)
+  | Callred (fd: fundef) (args: list val) (tyres: type) (m': mem).
+
+Section EXPRS.
+
+Variable e: env.
+
+Fixpoint sem_cast_arguments (vtl: list (val * type)) (tl: typelist) : option (list val) :=
+  match vtl, tl with
+  | nil, Tnil => Some nil
+  | (v1,t1)::vtl, Tcons t1' tl =>
+      do v <- sem_cast v1 t1 t1'; do vl <- sem_cast_arguments vtl tl; Some(v::vl)
+  | _, _ => None
+  end.
+
+(** The result of stepping an expression can be
+- [None] denoting that the expression is stuck;
+- [Some nil] meaning that the expression is fully reduced
+   (it's [Eval] for a r-value and [Eloc] for a l-value);
+- [Some ll] meaning that the expression can reduce to any of
+   the elements of [ll].  Each element is a pair of a context
+   and a reduction inside this context (see type [reduction] above).
+*)
+
+Definition reducts (A: Type): Type := option (list ((expr -> A) * reduction)).
+
+Definition topred (r: reduction) : reducts expr :=
+  Some (((fun (x: expr) => x), r) :: nil).
+
+Definition incontext {A B: Type} (ctx: A -> B) (r: reducts A) : reducts B :=
+  match r with
+  | None => None
+  | Some l => Some (map (fun z => ((fun (x: expr) => ctx(fst z x)), snd z)) l)
+  end.
+
+Definition incontext2 {A1 A2 B: Type}
+                     (ctx1: A1 -> B) (r1: reducts A1)
+                     (ctx2: A2 -> B) (r2: reducts A2) : reducts B :=
+  match r1, r2 with
+  | None, _ => None
+  | _, None => None
+  | Some l1, Some l2 =>
+      Some (map (fun z => ((fun (x: expr) => ctx1(fst z x)), snd z)) l1
+            ++ map (fun z => ((fun (x: expr) => ctx2(fst z x)), snd z)) l2)
+  end.
+
+Fixpoint step_expr (k: kind) (a: expr) (m: mem): reducts expr :=
+  match k, a with
+  | LV, Eloc b ofs ty =>
+      Some nil
+  | LV, Evar x ty =>
+      match e!x with
+      | Some(b, ty') =>
+          check type_eq ty ty';
+          topred (Lred (Eloc b Int.zero ty) m)
+      | None =>
+          do b <- Genv.find_symbol ge x;
+          do ty' <- type_of_global ge b;
+          check type_eq ty ty';
+          topred (Lred (Eloc b Int.zero ty) m)
+      end
+  | LV, Ederef r ty =>
+      match is_val r with
+      | Some(Vptr b ofs, ty') =>
+          topred (Lred (Eloc b ofs ty) m)
+      | Some _ =>
+          None
+      | None =>
+          incontext (fun x => Ederef x ty) (step_expr RV r m)
+      end
+  | LV, Efield l f ty =>
+      match is_loc l with
+      | Some(b, ofs, ty') =>
+          match ty' with
+          | Tstruct id fList =>
+              match field_offset f fList with
+              | Error _ => None
+              | OK delta => topred (Lred (Eloc b (Int.add ofs (Int.repr delta)) ty) m)
+              end
+          | Tunion id fList =>
+              topred (Lred (Eloc b ofs ty) m)
+          | _ => None
+          end
+      | None =>
+          incontext (fun x => Efield x f ty) (step_expr LV l m)
+      end
+  | RV, Eval v ty =>
+      Some nil
+  | RV, Evalof l ty =>
+      match is_loc l with
+      | Some(b, ofs, ty') =>
+          check type_eq ty ty';
+          do v <- load_value_of_type ty m b ofs;
+          topred (Rred (Eval v ty) m)
+      | None =>
+          incontext (fun x => Evalof x ty) (step_expr LV l m)
+      end
+  | RV, Eaddrof l ty =>
+      match is_loc l with
+      | Some(b, ofs, ty') => topred (Rred (Eval (Vptr b ofs) ty) m)
+      | None => incontext (fun x => Eaddrof x ty) (step_expr LV l m)
+      end
+  | RV, Eunop op r1 ty =>
+      match is_val r1 with
+      | Some(v1, ty1) =>
+          do v <- sem_unary_operation op v1 ty1;
+          topred (Rred (Eval v ty) m)
+      | None =>
+          incontext (fun x => Eunop op x ty) (step_expr RV r1 m)
+      end
+  | RV, Ebinop op r1 r2 ty =>
+      match is_val r1, is_val r2 with
+      | Some(v1, ty1), Some(v2, ty2) =>
+          do v <- sem_binary_operation op v1 ty1 v2 ty2 m;
+          topred (Rred (Eval v ty) m)
+      | _, _ =>
+         incontext2 (fun x => Ebinop op x r2 ty) (step_expr RV r1 m)
+                    (fun x => Ebinop op r1 x ty) (step_expr RV r2 m)
+      end
+  | RV, Ecast r1 ty =>
+      match is_val r1 with
+      | Some(v1, ty1) =>
+          do v <- sem_cast v1 ty1 ty;
+          topred (Rred (Eval v ty) m)
+      | None =>
+          incontext (fun x => Ecast x ty) (step_expr RV r1 m)
+      end
+  | RV, Econdition r1 r2 r3 ty =>
+      match is_val r1 with
+      | Some(v1, ty1) =>
+          do b <- bool_val v1 ty1;
+          topred (Rred (Eparen (if b then r2 else r3) ty) m)
+      | None =>
+          incontext (fun x => Econdition x r2 r3 ty) (step_expr RV r1 m)
+      end
+  | RV, Esizeof ty' ty =>
+      topred (Rred (Eval (Vint (Int.repr (sizeof ty'))) ty) m)
+  | RV, Eassign l1 r2 ty =>
+      match is_loc l1, is_val r2 with
+      | Some(b, ofs, ty1), Some(v2, ty2) =>
+          check type_eq ty1 ty;
+          do v <- sem_cast v2 ty2 ty1;
+          do m' <- store_value_of_type ty1 m b ofs v;
+          topred (Rred (Eval v ty) m')
+      | _, _ =>
+         incontext2 (fun x => Eassign x r2 ty) (step_expr LV l1 m)
+                    (fun x => Eassign l1 x ty) (step_expr RV r2 m)
+      end
+  | RV, Eassignop op l1 r2 tyres ty =>
+      match is_loc l1, is_val r2 with
+      | Some(b, ofs, ty1), Some(v2, ty2) =>
+          check type_eq ty1 ty;
+          do v1 <- load_value_of_type ty1 m b ofs;
+          do v <- sem_binary_operation op v1 ty1 v2 ty2 m;
+          do v' <- sem_cast v tyres ty1;
+          do m' <- store_value_of_type ty1 m b ofs v';
+          topred (Rred (Eval v' ty) m')
+      | _, _ =>
+         incontext2 (fun x => Eassignop op x r2 tyres ty) (step_expr LV l1 m)
+                    (fun x => Eassignop op l1 x tyres ty) (step_expr RV r2 m)
+      end
+  | RV, Epostincr id l ty =>
+      match is_loc l with
+      | Some(b, ofs, ty1) =>
+          check type_eq ty1 ty;
+          do v1 <- load_value_of_type ty m b ofs;
+          do v2 <- sem_incrdecr id v1 ty;
+          do v3 <- sem_cast v2 (typeconv ty) ty;
+          do m' <- store_value_of_type ty m b ofs v3;
+          topred (Rred (Eval v1 ty) m')
+      | None =>
+          incontext (fun x => Epostincr id x ty) (step_expr LV l m)
+      end
+  | RV, Ecomma r1 r2 ty =>
+      match is_val r1 with
+      | Some _ =>
+          check type_eq (typeof r2) ty;
+          topred (Rred r2 m)
+      | None =>
+          incontext (fun x => Ecomma x r2 ty) (step_expr RV r1 m)
+      end
+  | RV, Eparen r1 ty =>
+      match is_val r1 with
+      | Some (v1, ty1) =>
+          do v <- sem_cast v1 ty1 ty;
+          topred (Rred (Eval v ty) m)
+      | None =>
+          incontext (fun x => Eparen x ty) (step_expr RV r1 m)
+      end
+  | RV, Ecall r1 rargs ty =>
+      match is_val r1, is_val_list rargs with
+      | Some(vf, tyf), Some vtl =>
+          match classify_fun tyf with
+          | fun_case_f tyargs tyres =>
+              do fd <- Genv.find_funct ge vf;
+              do vargs <- sem_cast_arguments vtl tyargs;
+              check type_eq (type_of_fundef fd) (Tfunction tyargs tyres);
+              topred (Callred fd vargs ty m)
+          | _ => None
+          end
+      | _, _ =>
+          incontext2 (fun x => Ecall x rargs ty) (step_expr RV r1 m)
+                     (fun x => Ecall r1 x ty) (step_exprlist rargs m)
+      end
+  | _, _ => None
+  end
+
+with step_exprlist (rl: exprlist) (m: mem): reducts exprlist :=
+  match rl with
+  | Enil =>
+      Some nil
+  | Econs r1 rs =>
+      incontext2 (fun x => Econs x rs) (step_expr RV r1 m)
+                 (fun x => Econs r1 x) (step_exprlist rs m)
+  end.
+
+(** Soundness: if [step_expr] returns [Some ll], then every element
+  of [ll] is a reduct. *)
+
+Lemma context_compose:
+  forall k2 k3 C2, context k2 k3 C2 ->
+  forall k1 C1, context k1 k2 C1 ->
+  context k1 k3 (fun x => C2(C1 x))
+with contextlist_compose:
+  forall k2 C2, contextlist k2 C2 ->
+  forall k1 C1, context k1 k2 C1 ->
+  contextlist k1 (fun x => C2(C1 x)).
+Proof.
+  induction 1; intros; try (constructor; eauto).
+  replace (fun x => C1 x) with C1. auto. apply extensionality; auto.
+  induction 1; intros; constructor; eauto.
+Qed.
+
+Hint Constructors context contextlist.
+Hint Resolve context_compose contextlist_compose.
+
+Definition reduction_ok (a: expr) (m: mem) (rd: reduction) : Prop :=
+  match rd with
+  | Lred l' m' => lred ge e a m l' m'
+  | Rred r' m' => rred a m r' m'
+  | Callred fd args tyres m' => callred ge a fd args tyres /\ m' = m
+  end.
+
+Definition reduction_kind (rd: reduction): kind :=
+  match rd with
+  | Lred l' m' => LV
+  | Rred r' m' => RV
+  | Callred fd args tyres m' => RV
+  end.
+
+Ltac monadInv :=
+  match goal with
+  | [ H: match ?x with Some _ => _ | None => None end = Some ?y |- _ ] =>
+      destruct x as []_eqn; [monadInv|discriminate]
+  | [ H: match ?x with left _ => _ | right _ => None end = Some ?y |- _ ] =>
+      destruct x; [monadInv|discriminate]
+  | _ => idtac
+  end.
+
+Lemma sem_cast_arguments_sound:
+  forall rargs vtl tyargs vargs,
+  is_val_list rargs = Some vtl ->
+  sem_cast_arguments vtl tyargs = Some vargs ->
+  cast_arguments rargs tyargs vargs.
+Proof.
+  induction rargs; simpl; intros.
+  inv H. destruct tyargs; simpl in H0; inv H0. constructor.
+  monadInv. inv H. simpl in H0. destruct p as [v1 t1]. destruct tyargs; try congruence. monadInv.
+  inv H0. rewrite (is_val_inv _ _ _ Heqo). constructor. auto. eauto. 
+Qed.
+
+Definition reducts_ok (k: kind) (a: expr) (m: mem) (res: reducts expr) : Prop :=
+  match res with
+  | None => True
+  | Some nil => match k with LV => is_loc a <> None | RV => is_val a <> None end
+  | Some ll =>
+      forall C rd,
+      In (C, rd) ll ->
+      context (reduction_kind rd) k C /\ exists a', a = C a' /\ reduction_ok a' m rd
+  end.
+
+Definition list_reducts_ok (al: exprlist) (m: mem) (res: reducts exprlist) : Prop :=
+  match res with
+  | None => True
+  | Some nil => is_val_list al <> None
+  | Some ll =>
+      forall C rd,
+      In (C, rd) ll ->
+      contextlist (reduction_kind rd) C /\ exists a', al = C a' /\ reduction_ok a' m rd
+  end.
+
+Lemma topred_ok:
+  forall k a m rd,
+  reduction_ok a m rd ->
+  k = reduction_kind rd ->
+  reducts_ok k a m (topred rd).
+Proof.
+  intros. unfold topred; red. simpl; intros. destruct H1; try contradiction.
+  inv H1. split. auto. exists a; auto.
+Qed.
+
+Lemma incontext_ok:
+  forall k a m C res k' a',
+  reducts_ok k' a' m res ->
+  a = C a' ->
+  context k' k C ->
+  match k' with LV => is_loc a' = None | RV => is_val a' = None end ->
+  reducts_ok k a m (incontext C res).
+Proof.
+  unfold reducts_ok; intros. destruct res; simpl. destruct l.
+(* res = Some nil *)
+  destruct k'; congruence.
+(* res = Some nonempty-list *)
+  simpl map at 1. hnf. intros. 
+  exploit list_in_map_inv; eauto. intros [[C1 rd1] [P Q]]. inv P.
+  exploit H; eauto. intros [U [a'' [V W]]].
+  split. eapply context_compose; eauto. exists a''; split; auto. congruence. 
+(* res = None *)
+  auto.
+Qed.
+
+Remark incontext2_inv:
+  forall {A1 A2 B: Type} (C1: A1 -> B) res1 (C2: A2 -> B) res2,
+  match incontext2 C1 res1 C2 res2 with
+  | None => res1 = None \/ res2 = None
+  | Some nil => res1 = Some nil /\ res2 = Some nil
+  | Some ll => 
+      exists ll1, exists ll2,
+      res1 = Some ll1 /\ res2 = Some ll2 /\
+      forall C rd, In (C, rd) ll ->
+      (exists C', C = (fun x => C1(C' x)) /\ In (C', rd) ll1)
+      \/ (exists C', C = (fun x => C2(C' x)) /\ In (C', rd) ll2)
+  end.
+Proof.
+  intros. unfold incontext2. destruct res1 as [ll1|]; auto. destruct res2 as [ll2|]; auto.
+  set (ll := map
+    (fun z : (expr -> A1) * reduction =>
+     (fun x : expr => C1 (fst z x), snd z)) ll1 ++
+  map
+    (fun z : (expr -> A2) * reduction =>
+     (fun x : expr => C2 (fst z x), snd z)) ll2).
+  destruct ll as []_eqn.
+  destruct (app_eq_nil _ _ Heql). 
+  split. destruct ll1; auto || discriminate. destruct ll2; auto || discriminate.
+  rewrite <- Heql. exists ll1; exists ll2. split. auto. split. auto.
+  unfold ll; intros.
+  rewrite in_app in H. destruct H.
+  exploit list_in_map_inv; eauto. intros [[C' rd'] [P Q]]. inv P.
+  left; exists C'; auto. 
+  exploit list_in_map_inv; eauto. intros [[C' rd'] [P Q]]. inv P.
+  right; exists C'; auto.
+Qed.
+
+Lemma incontext2_ok:
+  forall k a m k1 a1 res1 k2 a2 res2 C1 C2,
+  reducts_ok k1 a1 m res1 ->
+  reducts_ok k2 a2 m res2 ->
+  a = C1 a1 -> a = C2 a2 ->
+  context k1 k C1 -> context k2 k C2 ->
+  match k1 with LV => is_loc a1 = None | RV => is_val a1 = None end
+  \/ match k2 with LV => is_loc a2 = None | RV => is_val a2 = None end ->
+  reducts_ok k a m (incontext2 C1 res1 C2 res2).
+Proof.
+  unfold reducts_ok; intros.
+  generalize (incontext2_inv C1 res1 C2 res2). 
+  destruct (incontext2 C1 res1 C2 res2) as [ll|]; auto.
+  destruct ll. 
+  intros [EQ1 EQ2]. subst. destruct H5. destruct k1; congruence. destruct k2; congruence.
+  intros [ll1 [ll2 [EQ1 [EQ2 IN]]]]. subst. intros. 
+  exploit IN; eauto. intros [[C' [P Q]] | [C' [P Q]]]; subst.
+  destruct ll1; try contradiction. exploit H; eauto.
+  intros [U [a' [V W]]]. split. eauto. exists a'; split. congruence. auto. 
+  destruct ll2; try contradiction. exploit H0; eauto.
+  intros [U [a' [V W]]]. split. eauto. exists a'; split. congruence. auto.
+Qed.
+
+Lemma incontext2_list_ok:
+  forall a1 a2 ty m res1 res2,
+  reducts_ok RV a1 m res1 ->
+  list_reducts_ok a2 m res2 ->
+  is_val a1 = None \/ is_val_list a2 = None ->
+  reducts_ok RV (Ecall a1 a2 ty) m 
+               (incontext2 (fun x => Ecall x a2 ty) res1
+                           (fun x => Ecall a1 x ty) res2).
+Proof.
+  unfold reducts_ok, list_reducts_ok; intros.
+  set (C1 := fun x => Ecall x a2 ty). set (C2 := fun x => Ecall a1 x ty). 
+  generalize (incontext2_inv C1 res1 C2 res2). 
+  destruct (incontext2 C1 res1 C2 res2) as [ll|]; auto.
+  destruct ll. 
+  intros [EQ1 EQ2]. subst. intuition congruence.
+  intros [ll1 [ll2 [EQ1 [EQ2 IN]]]]. subst. intros. 
+  exploit IN; eauto. intros [[C' [P Q]] | [C' [P Q]]]; subst.
+  destruct ll1; try contradiction. exploit H; eauto.
+  intros [U [a' [V W]]]. split. unfold C1. auto. exists a'; split. unfold C1; congruence. auto. 
+  destruct ll2; try contradiction. exploit H0; eauto.
+  intros [U [a' [V W]]]. split. unfold C2. auto. exists a'; split. unfold C2; congruence. auto.
+Qed.
+
+Lemma incontext2_list_ok':
+  forall a1 a2 m res1 res2,
+  reducts_ok RV a1 m res1 ->
+  list_reducts_ok a2 m res2 ->
+  list_reducts_ok (Econs a1 a2) m
+               (incontext2 (fun x => Econs x a2) res1
+                           (fun x => Econs a1 x) res2).
+Proof.
+  unfold reducts_ok, list_reducts_ok; intros.
+  set (C1 := fun x => Econs x a2). set (C2 := fun x => Econs a1 x). 
+  generalize (incontext2_inv C1 res1 C2 res2). 
+  destruct (incontext2 C1 res1 C2 res2) as [ll|]; auto.
+  destruct ll. 
+  intros [EQ1 EQ2]. subst.
+  simpl. destruct (is_val a1); try congruence. destruct (is_val_list a2); congruence.
+  intros [ll1 [ll2 [EQ1 [EQ2 IN]]]]. subst. intros. 
+  exploit IN; eauto. intros [[C' [P Q]] | [C' [P Q]]]; subst.
+  destruct ll1; try contradiction. exploit H; eauto.
+  intros [U [a' [V W]]]. split. unfold C1. auto. exists a'; split. unfold C1; congruence. auto. 
+  destruct ll2; try contradiction. exploit H0; eauto.
+  intros [U [a' [V W]]]. split. unfold C2. auto. exists a'; split. unfold C2; congruence. auto.
+Qed.
+
+Ltac mysimpl :=
+  match goal with
+  | [ |- reducts_ok _ _ _ (match ?x with Some _ => _ | None => None end) ] =>
+      destruct x as []_eqn; [mysimpl|exact I]
+  | [ |- reducts_ok _ _ _ (match ?x with left _ => _ | right _ => None end) ] =>
+      destruct x as []_eqn; [subst;mysimpl|exact I]
+  | _ =>
+      idtac
+  end.
+
+Theorem step_expr_sound:
+  forall a k m, reducts_ok k a m (step_expr k a m)
+with step_exprlist_sound:
+  forall al m, list_reducts_ok al m (step_exprlist al m).
+Proof with try (exact I).
+  induction a; destruct k; intros; simpl...
+(* Eval *)
+  congruence.
+(* Evar *)
+  destruct (e!x) as [[b ty'] | ]_eqn; mysimpl.
+  apply topred_ok; auto. apply red_var_local; auto.
+  apply topred_ok; auto. apply red_var_global; auto.
+(* Efield *)
+  destruct (is_loc a) as [[[b ofs] ty'] | ]_eqn.
+  destruct ty'... 
+  (* top struct *)
+  destruct (field_offset f f0) as [delta|]_eqn...
+  rewrite (is_loc_inv _ _ _ _ Heqo). apply topred_ok; auto. apply red_field_struct; auto.
+  (* top union *)
+  rewrite (is_loc_inv _ _ _ _ Heqo). apply topred_ok; auto. apply red_field_union; auto.
+  (* in depth *)
+  eapply incontext_ok; eauto. 
+(* Evalof *)
+  destruct (is_loc a) as [[[b ofs] ty'] | ]_eqn.
+  (* top *)
+  mysimpl. apply topred_ok; auto. rewrite (is_loc_inv _ _ _ _ Heqo). apply red_rvalof; auto. 
+  (* depth *)
+  eapply incontext_ok; eauto.
+(* Ederef *)
+  destruct (is_val a) as [[v ty'] | ]_eqn.
+  (* top *)
+  destruct v... mysimpl. apply topred_ok; auto. rewrite (is_val_inv _ _ _ Heqo). apply red_deref; auto. 
+  (* depth *)
+  eapply incontext_ok; eauto.
+(* Eaddrof *)
+  destruct (is_loc a) as [[[b ofs] ty'] | ]_eqn.
+  (* top *)
+  apply topred_ok; auto. rewrite (is_loc_inv _ _ _ _ Heqo). apply red_addrof; auto. 
+  (* depth *)
+  eapply incontext_ok; eauto.
+(* unop *)
+  destruct (is_val a) as [[v ty'] | ]_eqn.
+  (* top *)
+  mysimpl. apply topred_ok; auto. rewrite (is_val_inv _ _ _ Heqo). apply red_unop; auto. 
+  (* depth *)
+  eapply incontext_ok; eauto.
+(* binop *)
+  destruct (is_val a1) as [[v1 ty1] | ]_eqn.
+  destruct (is_val a2) as [[v2 ty2] | ]_eqn.
+  (* top *)
+  mysimpl. apply topred_ok; auto. 
+  rewrite (is_val_inv _ _ _ Heqo). rewrite (is_val_inv _ _ _ Heqo0). apply red_binop; auto.
+  (* depth *)
+  eapply incontext2_ok; eauto. 
+  eapply incontext2_ok; eauto. 
+(* cast *)
+  destruct (is_val a) as [[v ty'] | ]_eqn.
+  (* top *)
+  mysimpl. apply topred_ok; auto. 
+  rewrite (is_val_inv _ _ _ Heqo). apply red_cast; auto. 
+  (* depth *)
+  eapply incontext_ok; eauto.
+(* condition *)
+  destruct (is_val a1) as [[v ty'] | ]_eqn.
+  (* top *)
+  mysimpl. apply topred_ok; auto.
+  rewrite (is_val_inv _ _ _ Heqo). eapply red_condition; eauto.
+  (* depth *)
+  eapply incontext_ok; eauto.
+(* sizeof *)
+  apply topred_ok; auto. apply red_sizeof.
+(* assign *)
+  destruct (is_loc a1) as [[[b ofs] ty1] | ]_eqn.
+  destruct (is_val a2) as [[v2 ty2] | ]_eqn.
+  (* top *)
+  mysimpl. apply topred_ok; auto.
+  rewrite (is_loc_inv _ _ _ _ Heqo). rewrite (is_val_inv _ _ _ Heqo0). apply red_assign; auto.
+  (* depth *)
+  eapply incontext2_ok; eauto.
+  eapply incontext2_ok; eauto.
+(* assignop *)
+  destruct (is_loc a1) as [[[b ofs] ty1] | ]_eqn.
+  destruct (is_val a2) as [[v2 ty2] | ]_eqn.
+  (* top *)
+  mysimpl. apply topred_ok; auto.
+  rewrite (is_loc_inv _ _ _ _ Heqo). rewrite (is_val_inv _ _ _ Heqo0). eapply red_assignop; eauto.
+  (* depth *)
+  eapply incontext2_ok; eauto.
+  eapply incontext2_ok; eauto.
+(* postincr *)
+  destruct (is_loc a) as [[[b ofs] ty'] | ]_eqn.
+  (* top *)
+  mysimpl. apply topred_ok; auto.
+  rewrite (is_loc_inv _ _ _ _ Heqo). eapply red_postincr; eauto. 
+  (* depth *)
+  eapply incontext_ok; eauto.
+(* comma *)
+  destruct (is_val a1) as [[v ty'] | ]_eqn.
+  (* top *)
+  mysimpl. apply topred_ok; auto.
+  rewrite (is_val_inv _ _ _ Heqo). apply red_comma; auto. 
+  (* depth *)
+  eapply incontext_ok; eauto.
+(* call *)
+  destruct (is_val a) as [[vf tyf] | ]_eqn.
+  destruct (is_val_list rargs) as [vtl | ]_eqn.
+  (* top *)
+  destruct (classify_fun tyf) as [tyargs tyres|]_eqn...
+  mysimpl. apply topred_ok; auto.
+  rewrite (is_val_inv _ _ _ Heqo). red. split; auto. eapply red_Ecall; eauto. 
+  eapply sem_cast_arguments_sound; eauto. 
+  (* depth *)
+  eapply incontext2_list_ok; eauto.
+  eapply incontext2_list_ok; eauto. 
+(* loc *)
+  congruence.
+(* paren *)
+  destruct (is_val a) as [[v ty'] | ]_eqn.
+  (* top *)
+  mysimpl. apply topred_ok; auto.
+  rewrite (is_val_inv _ _ _ Heqo). apply red_paren; auto. 
+  (* depth *)
+  eapply incontext_ok; eauto.
+
+  induction al; simpl; intros.
+(* nil *)
+  congruence.
+(* cons *)
+  eapply incontext2_list_ok'; eauto.
+Qed.
+
+
+Lemma step_exprlist_val_list:
+  forall m al, is_val_list al <> None -> step_exprlist al m = Some nil.
+Proof.
+  induction al; simpl; intros. 
+  auto.
+  destruct (is_val r1) as [[v1 ty1]|]_eqn; try congruence.
+  destruct (is_val_list al) as []_eqn; try congruence.
+  rewrite (is_val_inv _ _ _ Heqo).
+  rewrite IHal. auto. congruence.
+Qed.
+
+(** Completeness, part 1: if [step_expr] returns [Some ll],
+  then [ll] contains all possible reducts. *)
+
+Lemma lred_topred:
+  forall l1 m1 l2 m2,
+  lred ge e l1 m1 l2 m2 ->
+  step_expr LV l1 m1 = topred (Lred l2 m2).
+Proof.
+  induction 1; simpl.
+(* var local *)
+  rewrite H. rewrite dec_eq_true; auto.
+(* var global *)
+  rewrite H; rewrite H0; rewrite H1. rewrite dec_eq_true; auto.
+(* deref *) 
+  auto.
+(* field struct *)
+  rewrite H; auto.
+(* field union *)
+  auto.
+Qed.
+
+Lemma rred_topred:
+  forall r1 m1 r2 m2,
+  rred r1 m1 r2 m2 ->
+  step_expr RV r1 m1 = topred (Rred r2 m2).
+Proof.
+  induction 1; simpl.
+(* valof *)
+  rewrite dec_eq_true; auto. rewrite H; auto.
+(* addrof *)
+  auto.
+(* unop *)
+  rewrite H; auto.
+(* binop *)
+  rewrite H; auto.
+(* cast *)
+  rewrite H; auto.
+(* condition *)
+  rewrite H; auto.
+(* sizeof *)
+  auto.
+(* assign *)
+  rewrite dec_eq_true; auto. rewrite H; rewrite H0; auto.
+(* assignop *)
+  rewrite dec_eq_true; auto. rewrite H; rewrite H0; rewrite H1; rewrite H2; auto.
+(* postincr *)
+  rewrite dec_eq_true; auto. rewrite H; rewrite H0; rewrite H1; rewrite H2; auto.
+(* comma *)
+  rewrite H; rewrite dec_eq_true; auto.
+(* paren *)
+  rewrite H; auto.
+Qed.
+
+Lemma sem_cast_arguments_complete:
+  forall al tyl vl,
+  cast_arguments al tyl vl ->
+  exists vtl, is_val_list al = Some vtl /\ sem_cast_arguments vtl tyl = Some vl.
+Proof.
+  induction 1.
+  exists (@nil (val * type)); auto.
+  destruct IHcast_arguments as [vtl [A B]]. 
+  exists ((v, ty) :: vtl); simpl. rewrite A; rewrite B; rewrite H. auto.
+Qed.
+
+Lemma callred_topred:
+  forall a fd args ty m,
+  callred ge a fd args ty ->
+  step_expr RV a m = topred (Callred fd args ty m).
+Proof.
+  induction 1; simpl.
+  rewrite H2. exploit sem_cast_arguments_complete; eauto. intros [vtl [A B]].
+  rewrite A; rewrite H; rewrite B; rewrite H1; rewrite dec_eq_true. auto.
+Qed.
+
+Definition reducts_incl {A B: Type} (C: A -> B) (res1: reducts A) (res2: reducts B) : Prop :=
+  match res1, res2 with
+  | Some ll1, Some ll2 =>
+      forall C1 rd, In (C1, rd) ll1 -> In ((fun x => C(C1 x)), rd) ll2
+  | None, Some ll2 => False
+  | _, None => True
+  end.
+
+Lemma reducts_incl_trans:
+  forall (A1 A2: Type) (C: A1 -> A2) res1 res2, reducts_incl C res1 res2 ->
+  forall (A3: Type) (C': A2 -> A3) res3,
+  reducts_incl C' res2 res3 ->
+  reducts_incl (fun x => C'(C x)) res1 res3.
+Proof.
+  unfold reducts_incl; intros. destruct res1; destruct res2; destruct res3; auto. contradiction.
+Qed.
+
+Lemma reducts_incl_nil:
+  forall (A B: Type) (C: A -> B) res,
+  reducts_incl C (Some nil) res.
+Proof.
+  intros; red. destruct res; auto. intros; contradiction.
+Qed.
+
+Lemma reducts_incl_val:
+  forall (A: Type) a m v ty (C: expr -> A) res,
+  is_val a = Some(v, ty) -> reducts_incl C (step_expr RV a m) res.
+Proof.
+  intros. rewrite (is_val_inv _ _ _ H). apply reducts_incl_nil.
+Qed.
+
+Lemma reducts_incl_loc:
+  forall (A: Type) a m b ofs ty (C: expr -> A) res,
+  is_loc a = Some(b, ofs, ty) -> reducts_incl C (step_expr LV a m) res.
+Proof.
+  intros. rewrite (is_loc_inv _ _ _ _ H). apply reducts_incl_nil.
+Qed.
+
+Lemma reducts_incl_listval:
+  forall (A: Type) a m vtl (C: exprlist -> A) res,
+  is_val_list a = Some vtl -> reducts_incl C (step_exprlist a m) res.
+Proof.
+  intros. rewrite step_exprlist_val_list. apply reducts_incl_nil. congruence.
+Qed.
+
+Lemma reducts_incl_incontext:
+  forall (A B: Type) (C: A -> B) res,
+  reducts_incl C res (incontext C res).
+Proof.
+  intros; unfold reducts_incl. destruct res; simpl; auto.
+  intros. set (f := fun z : (expr -> A) * reduction => (fun x : expr => C (fst z x), snd z)).
+  change (In (f (C1, rd)) (map f l)). apply in_map. auto.
+Qed.
+
+Lemma reducts_incl_incontext2_left:
+  forall (A1 A2 B: Type) (C1: A1 -> B) res1 (C2: A2 -> B) res2,
+  reducts_incl C1 res1 (incontext2 C1 res1 C2 res2).
+Proof.
+  intros. destruct res1; simpl; auto. destruct res2; auto. 
+  intros. rewrite in_app_iff. left.
+  set (f := fun z : (expr -> A1) * reduction => (fun x : expr => C1 (fst z x), snd z)).
+  change (In (f (C0, rd)) (map f l)). apply in_map; auto.
+Qed.
+
+Lemma reducts_incl_incontext2_right:
+  forall (A1 A2 B: Type) (C1: A1 -> B) res1 (C2: A2 -> B) res2,
+  reducts_incl C2 res2 (incontext2 C1 res1 C2 res2).
+Proof.
+  intros. destruct res1; destruct res2; simpl; auto.
+  intros. rewrite in_app_iff. right.
+  set (f := fun z : (expr -> A2) * reduction => (fun x : expr => C2 (fst z x), snd z)).
+  change (In (f (C0, rd)) (map f l0)). apply in_map; auto.
+Qed.
+
+Hint Resolve reducts_incl_val reducts_incl_loc reducts_incl_listval
+             reducts_incl_incontext reducts_incl_incontext2_left reducts_incl_incontext2_right.
+
+Lemma step_expr_context:
+  forall from to C, context from to C ->
+  forall a m, reducts_incl C (step_expr from a m) (step_expr to (C a) m)
+with step_exprlist_context:
+  forall from C, contextlist from C ->
+  forall a m, reducts_incl C (step_expr from a m) (step_exprlist (C a) m).
+Proof.
+  induction 1; simpl; intros.
+(* top *)
+  red. destruct (step_expr k a m); auto. intros. 
+  replace (fun x => C1 x) with C1; auto. apply extensionality; auto.
+(* deref *)
+  eapply reducts_incl_trans with (C' := fun x => Ederef x ty); eauto.
+  destruct (is_val (C a)) as [[v ty']|]_eqn; eauto.
+(* field *)
+  eapply reducts_incl_trans with (C' := fun x => Efield x f ty); eauto.
+  destruct (is_loc (C a)) as [[[b ofs] ty']|]_eqn; eauto.
+(* valof *)
+  eapply reducts_incl_trans with (C' := fun x => Evalof x ty); eauto.
+  destruct (is_loc (C a)) as [[[b ofs] ty']|]_eqn; eauto.
+(* addrof *)
+  eapply reducts_incl_trans with (C' := fun x => Eaddrof x ty); eauto.
+  destruct (is_loc (C a)) as [[[b ofs] ty']|]_eqn; eauto.
+(* unop *)
+  eapply reducts_incl_trans with (C' := fun x => Eunop op x ty); eauto.
+  destruct (is_val (C a)) as [[v ty']|]_eqn; eauto.
+(* binop left *)
+  eapply reducts_incl_trans with (C' := fun x => Ebinop op x e2 ty); eauto.
+  destruct (is_val (C a)) as [[v ty']|]_eqn; eauto.
+(* binop right *)
+  eapply reducts_incl_trans with (C' := fun x => Ebinop op e1 x ty); eauto.
+  destruct (is_val e1) as [[v1 ty1]|]_eqn; eauto.
+  destruct (is_val (C a)) as [[v2 ty2]|]_eqn; eauto.
+(* cast *)
+  eapply reducts_incl_trans with (C' := fun x => Ecast x ty); eauto.
+  destruct (is_val (C a)) as [[v ty']|]_eqn; eauto.
+(* condition *)
+  eapply reducts_incl_trans with (C' := fun x => Econdition x r2 r3 ty); eauto.
+  destruct (is_val (C a)) as [[v ty']|]_eqn; eauto.
+(* assign left *)
+  eapply reducts_incl_trans with (C' := fun x => Eassign x e2 ty); eauto.
+  destruct (is_loc (C a)) as [[[b ofs] ty']|]_eqn; eauto.
+(* assign right *)
+  eapply reducts_incl_trans with (C' := fun x => Eassign e1 x ty); eauto.
+  destruct (is_loc e1) as [[[b ofs] ty1]|]_eqn; eauto.
+  destruct (is_val (C a)) as [[v2 ty2]|]_eqn; eauto.
+(* assignop left *)
+  eapply reducts_incl_trans with (C' := fun x => Eassignop op x e2 tyres ty); eauto.
+  destruct (is_loc (C a)) as [[[b ofs] ty']|]_eqn; eauto.
+(* assignop right *)
+  eapply reducts_incl_trans with (C' := fun x => Eassignop op e1 x tyres ty); eauto.
+  destruct (is_loc e1) as [[[b ofs] ty1]|]_eqn; eauto.
+  destruct (is_val (C a)) as [[v2 ty2]|]_eqn; eauto.
+(* postincr *)
+  eapply reducts_incl_trans with (C' := fun x => Epostincr id x ty); eauto.
+  destruct (is_loc (C a)) as [[[b ofs] ty']|]_eqn; eauto.
+(* call left *)
+  eapply reducts_incl_trans with (C' := fun x => Ecall x el ty); eauto.
+  destruct (is_val (C a)) as [[v ty']|]_eqn; eauto.
+(* call right *)
+  eapply reducts_incl_trans with (C' := fun x => Ecall e1 x ty). apply step_exprlist_context. auto. 
+  destruct (is_val e1) as [[v1 ty1]|]_eqn; eauto.
+  destruct (is_val_list (C a)) as [vl|]_eqn; eauto.
+(* comma *)
+  eapply reducts_incl_trans with (C' := fun x => Ecomma x e2 ty); eauto.
+  destruct (is_val (C a)) as [[v ty']|]_eqn; eauto.
+(* paren *)
+  eapply reducts_incl_trans with (C' := fun x => Eparen x ty); eauto.
+  destruct (is_val (C a)) as [[v ty']|]_eqn; eauto.
+
+  induction 1; simpl; intros.
+(* cons left *)
+  eapply reducts_incl_trans with (C' := fun x => Econs x el).
+  apply step_expr_context; eauto. eauto.
+(* binop right *)
+  eapply reducts_incl_trans with (C' := fun x => Econs e1 x).
+  apply step_exprlist_context; eauto. eauto.
+Qed.
+
+(** Completeness, part 2: given a safe expression, [step_expr] does not return [None]. *)
+
+Lemma topred_none:
+  forall rd, topred rd <> None.
+Proof.
+  intros; unfold topred; congruence.
+Qed.
+
+Lemma incontext_none:
+  forall (A B: Type) (C: A -> B) rds,
+  rds <> None -> incontext C rds <> None.
+Proof.
+  unfold incontext; intros. destruct rds; congruence.
+Qed.
+
+Lemma incontext2_none:
+  forall (A1 A2 B: Type) (C1: A1 -> B) rds1 (C2: A2 -> B) rds2,
+  rds1 <> None -> rds2 <> None -> incontext2 C1 rds1 C2 rds2 <> None.
+Proof.
+  unfold incontext2; intros. destruct rds1; destruct rds2; congruence.
+Qed.
+
+Lemma safe_expr_kind:
+  forall k C a m,
+  context k RV C ->
+  not_stuck ge e (C a) m ->
+  k = Cstrategy.expr_kind a.
+Proof.
+  intros.
+  symmetry. eapply Cstrategy.not_imm_stuck_kind; eauto.
+Qed.
+
+Lemma safe_inversion:
+  forall k C a m,
+  context k RV C ->
+  not_stuck ge e (C a) m ->
+  match a with
+  | Eloc _ _ _ => True
+  | Eval _ _ => True
+  | _ => Cstrategy.invert_expr_prop ge e a m
+  end.
+Proof.
+  intros. eapply Cstrategy.not_imm_stuck_inv; eauto.
+Qed. 
+
+Lemma is_val_list_all_values:
+  forall al vtl, is_val_list al = Some vtl -> Cstrategy.exprlist_all_values al.
+Proof.
+  induction al; simpl; intros. auto. 
+  destruct (is_val r1) as [[v ty]|]_eqn; try discriminate.
+  destruct (is_val_list al) as [vtl'|]_eqn; try discriminate.
+  rewrite (is_val_inv _ _ _ Heqo). eauto.
+Qed.
+
+Theorem step_expr_defined:
+  forall a k m C,
+  context k RV C ->
+  not_stuck ge e (C a) m ->
+  step_expr k a m <> None
+with step_exprlist_defined:
+  forall al m C,
+  Cstrategy.contextlist' C ->
+  not_stuck ge e (C al) m ->
+  step_exprlist al m <> None.
+Proof.
+  induction a; intros k m C CTX NS; 
+  rewrite (safe_expr_kind _ _ _ _ CTX NS);
+  rewrite (safe_expr_kind _ _ _ _ CTX NS) in CTX;
+  simpl in *;
+  generalize (safe_inversion _ _ _ _ CTX NS); intro INV.
+(* val *)
+  congruence.
+(* var *)
+  red in INV. destruct INV as [b [P | [P [Q R]]]].
+  rewrite P; rewrite dec_eq_true. apply topred_none.
+  rewrite P; rewrite Q; rewrite R; rewrite dec_eq_true. apply topred_none.
+(* field *)
+  destruct (is_loc a) as [[[b ofs] ty']|]_eqn. 
+  rewrite (is_loc_inv _ _ _ _ Heqo) in INV. red in INV. 
+  destruct ty'; try contradiction. destruct INV as [delta EQ]. rewrite EQ. apply topred_none.
+  apply topred_none.
+  apply incontext_none. apply IHa with (C := fun x => C(Efield x f ty)); eauto.
+(* valof *)
+  destruct (is_loc a) as [[[b ofs] ty']|]_eqn. 
+  rewrite (is_loc_inv _ _ _ _ Heqo) in INV. red in INV. destruct INV as [EQ [v LD]]. subst.
+  rewrite dec_eq_true; rewrite LD; apply topred_none.
+  apply incontext_none. apply IHa with (C := fun x => C(Evalof x ty)); eauto.
+(* deref *)
+  destruct (is_val a) as [[v ty']|]_eqn. 
+  rewrite (is_val_inv _ _ _ Heqo) in INV. red in INV. destruct INV as [b [ofs EQ]]. subst. 
+  apply topred_none.
+  apply incontext_none. apply IHa with (C := fun x => C(Ederef x ty)); eauto.
+(* addrof *) 
+  destruct (is_loc a) as [[[b ofs] ty']|]_eqn. 
+  apply topred_none.
+  apply incontext_none. apply IHa with (C := fun x => C(Eaddrof x ty)); eauto.
+(* unop *)
+  destruct (is_val a) as [[v1 ty1]|]_eqn. 
+  rewrite (is_val_inv _ _ _ Heqo) in INV. red in INV. destruct INV as [v EQ].
+  rewrite EQ; apply topred_none.
+  apply incontext_none. apply IHa with (C := fun x => C(Eunop op x ty)); eauto.
+(* binop *)
+  destruct (is_val a1) as [[v1 ty1]|]_eqn. 
+  destruct (is_val a2) as [[v2 ty2]|]_eqn. 
+  rewrite (is_val_inv _ _ _ Heqo) in INV.
+  rewrite (is_val_inv _ _ _ Heqo0) in INV. red in INV. destruct INV as [v EQ].
+  rewrite EQ; apply topred_none.
+  apply incontext2_none. apply IHa1 with (C := fun x => C(Ebinop op x a2 ty)); eauto. apply IHa2 with (C := fun x => C(Ebinop op a1 x ty)); eauto.
+  apply incontext2_none. apply IHa1 with (C := fun x => C(Ebinop op x a2 ty)); eauto. apply IHa2 with (C := fun x => C(Ebinop op a1 x ty)); eauto.
+(* cast *)
+  destruct (is_val a) as [[v1 ty1]|]_eqn. 
+  rewrite (is_val_inv _ _ _ Heqo) in INV. red in INV. destruct INV as [v EQ].
+  rewrite EQ; apply topred_none.
+  apply incontext_none. apply IHa with (C := fun x => C(Ecast x ty)); eauto.
+(* condition *)
+  destruct (is_val a1) as [[v1 ty1]|]_eqn. 
+  rewrite (is_val_inv _ _ _ Heqo) in INV. red in INV. destruct INV as [v EQ].
+  rewrite EQ; apply topred_none.
+  apply incontext_none. apply IHa1 with (C := fun x => C(Econdition x a2 a3 ty)); eauto.
+(* sizeof *)
+  apply topred_none.
+(* assign *)
+  destruct (is_loc a1) as [[[b ofs] ty1]|]_eqn. 
+  destruct (is_val a2) as [[v2 ty2]|]_eqn. 
+  rewrite (is_loc_inv _ _ _ _ Heqo) in INV.
+  rewrite (is_val_inv _ _ _ Heqo0) in INV. red in INV. 
+  destruct INV as [v [m' [P [Q R]]]]. 
+  subst. rewrite dec_eq_true; rewrite Q; rewrite R; apply topred_none.
+  apply incontext2_none. apply IHa1 with (C := fun x => C(Eassign x a2 ty)); eauto. apply IHa2 with (C := fun x => C(Eassign a1 x ty)); eauto.
+  apply incontext2_none. apply IHa1 with (C := fun x => C(Eassign x a2 ty)); eauto. apply IHa2 with (C := fun x => C(Eassign a1 x ty)); eauto.
+(* assignop *)
+  destruct (is_loc a1) as [[[b ofs] ty1]|]_eqn. 
+  destruct (is_val a2) as [[v2 ty2]|]_eqn. 
+  rewrite (is_loc_inv _ _ _ _ Heqo) in INV.
+  rewrite (is_val_inv _ _ _ Heqo0) in INV. red in INV. 
+  destruct INV as [v1 [v [v' [m' [P [Q [R [S T]]]]]]]]. 
+  subst. rewrite dec_eq_true; rewrite Q; rewrite R; rewrite S; rewrite T; apply topred_none.
+  apply incontext2_none. apply IHa1 with (C := fun x => C(Eassignop op x a2 tyres ty)); eauto. apply IHa2 with (C := fun x => C(Eassignop op a1 x tyres ty)); eauto.
+  apply incontext2_none. apply IHa1 with (C := fun x => C(Eassignop op x a2 tyres ty)); eauto. apply IHa2 with (C := fun x => C(Eassignop op a1 x tyres ty)); eauto.
+(* postincr *)
+  destruct (is_loc a) as [[[b ofs] ty1]|]_eqn. 
+  rewrite (is_loc_inv _ _ _ _ Heqo) in INV. red in INV. 
+  destruct INV as [v1 [v2 [v3 [m' [P [Q [R [S T]]]]]]]]. 
+  subst. rewrite dec_eq_true; rewrite Q; rewrite R; rewrite S; rewrite T; apply topred_none.
+  apply incontext_none. apply IHa with (C := fun x => C(Epostincr id x ty)); eauto.
+(* comma *)
+  destruct (is_val a1) as [[v1 ty1]|]_eqn. 
+  rewrite (is_val_inv _ _ _ Heqo) in INV. red in INV. rewrite INV.
+  rewrite dec_eq_true; apply topred_none.
+  apply incontext_none. apply IHa1 with (C := fun x => C(Ecomma x a2 ty)); eauto.
+(* call *)
+  destruct (is_val a) as [[vf tyf]|]_eqn. 
+  destruct (is_val_list rargs) as [vtl|]_eqn. 
+  rewrite (is_val_inv _ _ _ Heqo) in INV. red in INV. 
+  destruct INV as [tyargs [tyres [fd [vl [P [Q [R S]]]]]]].
+  eapply is_val_list_all_values; eauto.
+  rewrite P; rewrite Q. 
+  exploit sem_cast_arguments_complete; eauto. intros [vtl' [U V]]. 
+  assert (vtl' = vtl) by congruence. subst. rewrite V. rewrite S. rewrite dec_eq_true. 
+  apply topred_none.
+  apply incontext2_none. apply IHa with (C := fun x => C(Ecall x rargs ty)); eauto.
+  apply step_exprlist_defined with (C := fun x => C(Ecall a x ty)); auto.
+  apply Cstrategy.contextlist'_intro with (rl0 := Enil). auto.
+  apply incontext2_none. apply IHa with (C := fun x => C(Ecall x rargs ty)); eauto.
+  apply step_exprlist_defined with (C := fun x => C(Ecall a x ty)); auto.
+  apply Cstrategy.contextlist'_intro with (rl0 := Enil). auto.
+(* loc *)
+  congruence.
+(* paren *)
+  destruct (is_val a) as [[v1 ty1]|]_eqn. 
+  rewrite (is_val_inv _ _ _ Heqo) in INV. red in INV. destruct INV as [v EQ].
+  rewrite EQ; apply topred_none.
+  apply incontext_none. apply IHa with (C := fun x => C(Eparen x ty)); eauto.
+
+  induction al; intros; simpl.
+(* nil *)
+  congruence.
+(* cons *)
+  apply incontext2_none.
+  apply step_expr_defined with (C := fun x => C(Econs x al)); eauto. 
+  apply Cstrategy.contextlist'_head; auto.
+  apply IHal with (C := fun x => C(Econs r1 x)); auto.
+  apply Cstrategy.contextlist'_tail; auto.
+Qed.
+
+(** Connections between [not_stuck] and [step_expr]. *)
+
+Lemma step_expr_not_imm_stuck:
+  forall k a m,
+  step_expr k a m <> None ->
+  not_imm_stuck ge e k a m.
+Proof.
+  intros. generalize (step_expr_sound a k m). unfold reducts_ok. 
+  destruct (step_expr k a m) as [ll|]. destruct ll.
+(* value or location *)
+  destruct k; destruct a; simpl; intros; try congruence. 
+  apply not_stuck_loc.
+  apply Csem.not_stuck_val.
+(* reducible *)
+  intros R. destruct p as [C1 rd1]. destruct (R C1 rd1) as [P [a' [U V]]]; auto with coqlib.
+  subst a. red in V. destruct rd1. 
+  eapply not_stuck_lred; eauto. 
+  eapply not_stuck_rred; eauto.
+  destruct V. subst m'. eapply not_stuck_callred; eauto.
+(* stuck *)
+  congruence.
+Qed.
+
+Lemma step_expr_not_stuck:
+  forall a m,
+  step_expr RV a m <> None ->
+  not_stuck ge e a m.
+Proof.
+  intros; red; intros. subst a. 
+  apply step_expr_not_imm_stuck.
+  generalize (step_expr_context _ _ C H0 e' m). unfold reducts_incl. 
+  destruct (step_expr k e' m). congruence.
+  destruct (step_expr RV (C e') m). tauto. congruence.
+Qed.
+
+Lemma not_stuck_step_expr:
+  forall a m,
+  not_stuck ge e a m ->
+  step_expr RV a m <> None.
+Proof.
+  intros. apply step_expr_defined with (C := fun x => x); auto. 
+Qed.
+
+End EXPRS.
+
+(** * External functions and events. *)
+
+Section EVENTS.
+
+Variable F V: Type.
+Variable genv: Genv.t F V.
+
+Definition eventval_of_val (v: val) (t: typ) : option eventval :=
+  match v, t with
+  | Vint i, AST.Tint => Some (EVint i)
+  | Vfloat f, AST.Tfloat => Some (EVfloat f)
+  | Vptr b ofs, AST.Tint => do id <- Genv.invert_symbol genv b; Some (EVptr_global id ofs)
+  | _, _ => None
+  end.
+
+Fixpoint list_eventval_of_val (vl: list val) (tl: list typ) : option (list eventval) :=
+  match vl, tl with
+  | nil, nil => Some nil
+  | v1::vl, t1::tl =>
+      do ev1 <- eventval_of_val v1 t1;
+      do evl <- list_eventval_of_val vl tl;
+      Some (ev1 :: evl)
+  | _, _ => None
+  end.
+
+Definition val_of_eventval (ev: eventval) (t: typ) : option val :=
+  match ev, t with
+  | EVint i, AST.Tint => Some (Vint i)
+  | EVfloat f, AST.Tfloat => Some (Vfloat f)
+  | EVptr_global id ofs, AST.Tint => do b <- Genv.find_symbol genv id; Some (Vptr b ofs)
+  | _, _ => None
+  end.
+
+Lemma eventval_of_val_sound:
+  forall v t ev, eventval_of_val v t = Some ev -> eventval_match genv ev t v.
+Proof.
+  intros. destruct v; destruct t; simpl in H; inv H.
+  constructor.
+  constructor.
+  destruct (Genv.invert_symbol genv b) as [id|]_eqn; inv H1. 
+  constructor. apply Genv.invert_find_symbol; auto.
+Qed.
+
+Lemma eventval_of_val_complete:
+  forall ev t v, eventval_match genv ev t v -> eventval_of_val v t = Some ev.
+Proof.
+  induction 1; simpl; auto.
+  rewrite (Genv.find_invert_symbol _ _ H). auto. 
+Qed.
+
+Lemma list_eventval_of_val_sound:
+  forall vl tl evl, list_eventval_of_val vl tl = Some evl -> eventval_list_match genv evl tl vl.
+Proof with try discriminate.
+  induction vl; destruct tl; simpl; intros; inv H.
+  constructor.
+  destruct (eventval_of_val a t) as [ev1|]_eqn...
+  destruct (list_eventval_of_val vl tl) as [evl'|]_eqn...
+  inv H1. constructor. apply eventval_of_val_sound; auto. eauto.
+Qed.
+
+Lemma list_eventval_of_val_complete:
+  forall evl tl vl, eventval_list_match genv evl tl vl -> list_eventval_of_val vl tl = Some evl.
+Proof.
+  induction 1; simpl. auto. 
+  rewrite (eventval_of_val_complete _ _ _ H). rewrite IHeventval_list_match. auto.
+Qed.
+
+Lemma val_of_eventval_sound:
+  forall ev t v, val_of_eventval ev t = Some v -> eventval_match genv ev t v.
+Proof.
+  intros. destruct ev; destruct t; simpl in H; inv H.
+  constructor.
+  constructor.
+  destruct (Genv.find_symbol genv i) as [b|]_eqn; inv H1.
+  constructor. auto.
+Qed.
+
+Lemma val_of_eventval_complete:
+  forall ev t v, eventval_match genv ev t v -> val_of_eventval ev t = Some v.
+Proof.
+  induction 1; simpl; auto. rewrite H; auto.
+Qed.
+
+(** System calls and library functions *)
+
+Definition do_ef_external (name: ident) (sg: signature)
+       (w: world) (vargs: list val) (m: mem) : option (world * trace * val * mem) :=
+  do args <- list_eventval_of_val vargs (sig_args sg);
+  match nextworld_io w name args with
+  | None => None
+  | Some(res, w') =>
+      do vres <- val_of_eventval res (proj_sig_res sg);
+      Some(w', Event_syscall name args res :: E0, vres, m)
+  end.
+
+Definition do_ef_volatile_load (chunk: memory_chunk)
+       (w: world) (vargs: list val) (m: mem) : option (world * trace * val * mem) :=
+  match vargs with
+  | Vptr b ofs :: nil =>
+      if block_is_volatile genv b then
+        do id <- Genv.invert_symbol genv b;
+        match nextworld_vload w chunk id ofs with
+        | None => None
+        | Some(res, w') =>
+            do vres <- val_of_eventval res (type_of_chunk chunk);
+            Some(w', Event_vload chunk id ofs res :: nil, Val.load_result chunk vres, m)
+        end
+      else
+        do v <- Mem.load chunk m b (Int.unsigned ofs);
+        Some(w, E0, v, m)
+  | _ => None
+  end.
+
+Definition do_ef_volatile_store (chunk: memory_chunk)
+       (w: world) (vargs: list val) (m: mem) : option (world * trace * val * mem) :=
+  match vargs with
+  | Vptr b ofs :: v :: nil =>
+      if block_is_volatile genv b then
+        do id <- Genv.invert_symbol genv b;
+        do ev <- eventval_of_val v (type_of_chunk chunk);
+        do w' <- nextworld_vstore w chunk id ofs ev;
+        Some(w', Event_vstore chunk id ofs ev :: nil, Vundef, m)
+      else
+        do m' <- Mem.store chunk m b (Int.unsigned ofs) v;
+        Some(w, E0, Vundef, m')
+  | _ => None
+  end.
+
+Definition do_ef_malloc
+       (w: world) (vargs: list val) (m: mem) : option (world * trace * val * mem) :=
+  match vargs with
+  | Vint n :: nil =>
+      let (m', b) := Mem.alloc m (-4) (Int.unsigned n) in
+      do m'' <- Mem.store Mint32 m' b (-4) (Vint n);
+      Some(w, E0, Vptr b Int.zero, m'')
+  | _ => None
+  end.
+
+Definition do_ef_free
+       (w: world) (vargs: list val) (m: mem) : option (world * trace * val * mem) :=
+  match vargs with
+  | Vptr b lo :: nil =>
+      do vsz <- Mem.load Mint32 m b (Int.unsigned lo - 4);
+      match vsz with
+      | Vint sz =>
+          check (zlt 0 (Int.unsigned sz));
+          do m' <- Mem.free m b (Int.unsigned lo - 4) (Int.unsigned lo + Int.unsigned sz);
+          Some(w, E0, Vundef, m')
+      | _ => None
+      end
+  | _ => None
+  end.
+
+Definition memcpy_args_ok
+  (sz al: Z) (bdst: block) (odst: Z) (bsrc: block) (osrc: Z) : Prop :=
+      (al = 1 \/ al = 2 \/ al = 4)
+   /\ sz > 0
+   /\ (al | sz) /\ (al | osrc) /\ (al | odst)
+   /\ (bsrc <> bdst \/ osrc = odst \/ osrc + sz <= odst \/ odst + sz <= osrc).
+
+Remark memcpy_check_args:
+  forall sz al bdst odst bsrc osrc,
+  {memcpy_args_ok sz al bdst odst bsrc osrc} + {~memcpy_args_ok sz al bdst odst bsrc osrc}.
+Proof with try (right; intuition omega).
+  intros. 
+  assert (X: {al = 1 \/ al = 2 \/ al = 4} + {~(al = 1 \/ al = 2 \/ al = 4)}).
+    destruct (zeq al 1); auto. destruct (zeq al 2); auto. destruct (zeq al 4); auto...
+  unfold memcpy_args_ok. destruct X...
+  assert (al > 0) by (intuition omega).
+  destruct (zlt 0 sz)...
+  destruct (Zdivide_dec al sz); auto...
+  destruct (Zdivide_dec al osrc); auto...
+  destruct (Zdivide_dec al odst); auto...
+  assert (Y: {bsrc <> bdst \/ osrc = odst \/ osrc + sz <= odst \/ odst + sz <= osrc}
+           +{~(bsrc <> bdst \/ osrc = odst \/ osrc + sz <= odst \/ odst + sz <= osrc)}).
+    destruct (eq_block bsrc bdst); auto.
+    destruct (zeq osrc odst); auto.
+    destruct (zle (osrc + sz) odst); auto.
+    destruct (zle (odst + sz) osrc); auto.
+    right; intuition omega.
+  destruct Y... left; intuition omega.
+Qed.
+
+Definition do_ef_memcpy (sz al: Z)
+       (w: world) (vargs: list val) (m: mem) : option (world * trace * val * mem) :=
+  match vargs with
+  | Vptr bdst odst :: Vptr bsrc osrc :: nil =>
+      if memcpy_check_args sz al bdst (Int.unsigned odst) bsrc (Int.unsigned osrc) then
+        do bytes <- Mem.loadbytes m bsrc (Int.unsigned osrc) sz;
+        do m' <- Mem.storebytes m bdst (Int.unsigned odst) bytes;
+        Some(w, E0, Vundef, m')
+      else None
+  | _ => None
+  end.
+
+Definition do_ef_annot (text: ident) (targs: list typ)
+       (w: world) (vargs: list val) (m: mem) : option (world * trace * val * mem) :=
+  do args <- list_eventval_of_val vargs targs;
+  Some(w, Event_annot text args :: E0, Vundef, m).
+
+Definition do_ef_annot_val (text: ident) (targ: typ)
+       (w: world) (vargs: list val) (m: mem) : option (world * trace * val * mem) :=
+  match vargs with
+  | varg :: nil =>
+      do arg <- eventval_of_val varg targ;
+      Some(w, Event_annot text (arg :: nil) :: E0, varg, m)
+  | _ => None
+  end.
+
+Definition do_external (ef: external_function):
+       world -> list val -> mem -> option (world * trace * val * mem) :=
+  match ef with
+  | EF_external name sg => do_ef_external name sg
+  | EF_builtin name sg => do_ef_external name sg
+  | EF_vload chunk => do_ef_volatile_load chunk
+  | EF_vstore chunk => do_ef_volatile_store chunk
+  | EF_malloc => do_ef_malloc
+  | EF_free => do_ef_free
+  | EF_memcpy sz al => do_ef_memcpy sz al
+  | EF_annot text targs => do_ef_annot text targs
+  | EF_annot_val text targ => do_ef_annot_val text targ
+  end.
+
+Ltac mydestr :=
+  match goal with
+  | [ |- None = Some _ -> _ ] => intro X; discriminate
+  | [ |- Some _ = Some _ -> _ ] => intro X; inv X
+  | [ |- match ?x with Some _ => _ | None => _ end = Some _ -> _ ] => destruct x as []_eqn; mydestr
+  | [ |- match ?x with true => _ | false => _ end = Some _ -> _ ] => destruct x as []_eqn; mydestr
+  | [ |- match ?x with left _ => _ | right _ => _ end = Some _ -> _ ] => destruct x; mydestr
+  | _ => idtac
+  end.
+
+Lemma do_ef_external_sound:
+  forall ef w vargs m w' t vres m',
+  do_external ef w vargs m = Some(w', t, vres, m') ->
+  external_call ef genv vargs m t vres m' /\ possible_trace w t w'.
+Proof with try congruence.
+  intros until m'.
+  assert (IO: forall name sg,
+             do_ef_external name sg w vargs m = Some(w', t, vres, m') ->
+             extcall_io_sem name sg genv vargs m t vres m' /\ possible_trace w t w').
+    intros until sg. unfold do_ef_external. mydestr. destruct p as [res w'']; mydestr.
+    split. econstructor. apply list_eventval_of_val_sound; auto. 
+    apply val_of_eventval_sound; auto. 
+    econstructor. constructor; eauto. constructor.
+
+  destruct ef; simpl.
+(* EF_external *)
+  auto. 
+(* EF_builtin *)
+  auto.
+(* EF_vload *)
+  unfold do_ef_volatile_load. destruct vargs... destruct v... destruct vargs... 
+  mydestr. destruct p as [res w'']; mydestr.
+  split. constructor. apply Genv.invert_find_symbol; auto. auto. 
+  apply val_of_eventval_sound; auto. 
+  econstructor. constructor; eauto. constructor.
+  split. constructor; auto. constructor.
+(* EF_vstore *)
+  unfold do_ef_volatile_store. destruct vargs... destruct v... destruct vargs... destruct vargs... 
+  mydestr.
+  split. constructor. apply Genv.invert_find_symbol; auto. auto. 
+  apply eventval_of_val_sound; auto. 
+  econstructor. constructor; eauto. constructor.
+  split. constructor; auto. constructor.
+(* EF_malloc *)
+  unfold do_ef_malloc. destruct vargs... destruct v... destruct vargs...
+  destruct (Mem.alloc m (-4) (Int.unsigned i)) as [m1 b]_eqn. mydestr.
+  split. econstructor; eauto. constructor.
+(* EF_free *)
+  unfold do_ef_free. destruct vargs... destruct v... destruct vargs... 
+  mydestr. destruct v... mydestr. 
+  split. econstructor; eauto. omega. constructor.
+(* EF_memcpy *)
+  unfold do_ef_memcpy. destruct vargs... destruct v... destruct vargs... 
+  destruct v... destruct vargs... mydestr. red in m0. 
+  split. econstructor; eauto; tauto. constructor.
+(* EF_annot *)
+  unfold do_ef_annot. mydestr. 
+  split. constructor. apply list_eventval_of_val_sound; auto.
+  econstructor. constructor; eauto. constructor.
+(* EF_annot_val *)
+  unfold do_ef_annot_val. destruct vargs... destruct vargs... mydestr. 
+  split. constructor. apply eventval_of_val_sound; auto.
+  econstructor. constructor; eauto. constructor.
+Qed.
+
+Lemma do_ef_external_complete:
+  forall ef w vargs m w' t vres m',
+  external_call ef genv vargs m t vres m' -> possible_trace w t w' ->
+  do_external ef w vargs m = Some(w', t, vres, m').
+Proof.
+  intros.
+  assert (IO: forall name sg,
+             extcall_io_sem name sg genv vargs m t vres m' ->
+             do_ef_external name sg w vargs m = Some (w', t, vres, m')).
+    intros. inv H1. inv H0. inv H8. inv H6. 
+    unfold do_ef_external. rewrite (list_eventval_of_val_complete _ _ _ H2). rewrite H8. 
+    rewrite (val_of_eventval_complete _ _ _ H3). auto.
+ 
+  destruct ef; simpl in *.
+(* EF_external *)
+  auto.
+(* EF_builtin *)
+  auto.
+(* EF_vload *)
+  inv H; unfold do_ef_volatile_load.
+  inv H0. inv H8. inv H6. 
+  rewrite H2. rewrite (Genv.find_invert_symbol _ _ H1). rewrite H9. 
+  rewrite (val_of_eventval_complete _ _ _ H3). auto.
+  inv H0. rewrite H1. rewrite H2. auto.
+(* EF_vstore *)
+  inv H; unfold do_ef_volatile_store.
+  inv H0. inv H8. inv H6. 
+  rewrite H2. rewrite (Genv.find_invert_symbol _ _ H1).
+  rewrite (eventval_of_val_complete _ _ _ H3). rewrite H9. auto.
+  inv H0. rewrite H1. rewrite H2. auto.
+(* EF_malloc *)
+  inv H; unfold do_ef_malloc. 
+  inv H0. rewrite H1. rewrite H2. auto.
+(* EF_free *)
+  inv H; unfold do_ef_free.
+  inv H0. rewrite H1. rewrite zlt_true. rewrite H3. auto. omega.
+(* EF_memcpy *)
+  inv H; unfold do_ef_memcpy.
+  inv H0. rewrite pred_dec_true. rewrite H7; rewrite H8; auto.
+  red. tauto. 
+(* EF_annot *)
+  inv H; unfold do_ef_annot. inv H0. inv H6. inv H4. 
+  rewrite (list_eventval_of_val_complete _ _ _ H1). auto.
+(* EF_annot_val *)
+  inv H; unfold do_ef_annot_val. inv H0. inv H6. inv H4. 
+  rewrite (eventval_of_val_complete _ _ _ H1). auto.
+Qed.
+
+End EVENTS.
+
+(** * Transitions over states. *)
+
+Fixpoint do_alloc_variables (e: env) (m: mem) (l: list (ident * type)) {struct l} : env * mem :=
+  match l with
+  | nil => (e,m)
+  | (id, ty) :: l' =>
+      let (m1,b1) := Mem.alloc m 0 (sizeof ty) in 
+      do_alloc_variables (PTree.set id (b1, ty) e) m1 l'
+end.
+
+Lemma do_alloc_variables_sound:
+  forall l e m, alloc_variables e m l (fst (do_alloc_variables e m l)) (snd (do_alloc_variables e m l)).
+Proof.
+  induction l; intros; simpl. 
+  constructor.
+  destruct a as [id ty]. destruct (Mem.alloc m 0 (sizeof ty)) as [m1 b1]_eqn; simpl.
+  econstructor; eauto.
+Qed.
+
+Lemma do_alloc_variables_complete:
+  forall e1 m1 l e2 m2, alloc_variables e1 m1 l e2 m2 ->
+  do_alloc_variables e1 m1 l = (e2, m2).
+Proof.
+  induction 1; simpl. 
+  auto.
+  rewrite H; rewrite IHalloc_variables; auto. 
+Qed.
+
+Function sem_bind_parameters (e: env) (m: mem) (l: list (ident * type)) (lv: list val) 
+                          {struct l} : option mem :=
+  match l, lv  with
+  | nil, nil => Some m
+  | (id, ty) :: params, v1::lv =>
+      match PTree.get id e with
+         | Some (b, ty') =>
+             check (type_eq ty ty');
+             do m1 <- store_value_of_type ty m b Int.zero v1;
+             sem_bind_parameters e m1 params lv
+        | None => None
+      end
+   | _, _ => None
+end.
+
+Lemma sem_bind_parameters_sound : forall e m l lv m',
+  sem_bind_parameters e m l lv = Some m' -> 
+  bind_parameters e m l lv m'.
+Proof.
+   intros; functional induction (sem_bind_parameters e m l lv); try discriminate.
+   inversion H; constructor; auto.  
+   econstructor; eauto.
+Qed.
+
+Lemma sem_bind_parameters_complete : forall e m l lv m',
+  bind_parameters e m l lv m' ->
+  sem_bind_parameters e m l lv = Some m'.
+Proof.
+   induction 1; simpl; auto.
+   rewrite H. rewrite dec_eq_true. 
+   destruct (store_value_of_type ty m b Int.zero v1); try discriminate.
+   inv H0; auto.
+Qed.
+
+Definition expr_final_state (f: function) (k: cont) (e: env) (C_rd: (expr -> expr) * reduction) :=
+  match snd C_rd with
+  | Lred a m => (E0, ExprState f (fst C_rd a) k e m)
+  | Rred a m => (E0, ExprState f (fst C_rd a) k e m)
+  | Callred fd vargs ty m => (E0, Callstate fd vargs (Kcall f e (fst C_rd) ty k) m)
+  end.
+
+Local Open Scope list_monad_scope.
+
+Definition ret (S: state) : list (trace * state) := (E0, S) :: nil.
+
+Definition do_step (w: world) (s: state) : list (trace * state) :=
+  match s with
+
+  | ExprState f a k e m =>
+      match is_val a with
+      | Some(v, ty) =>
+        match k with
+        | Kdo k => ret (State f Sskip k e m )
+        | Kifthenelse s1 s2 k =>
+            do b <- bool_val v ty; ret (State f (if b then s1 else s2) k e m)
+        | Kwhile1 x s k =>
+            do b <- bool_val v ty; 
+            if b then ret (State f s (Kwhile2 x s k) e m) else ret (State f Sskip k e m)
+        | Kdowhile2 x s k =>
+            do b <- bool_val v ty;
+            if b then ret (State f (Sdowhile x s) k e m) else ret (State f Sskip k e m)
+        | Kfor2 a2 a3 s k =>
+            do b <- bool_val v ty;
+            if b then ret (State f s (Kfor3 a2 a3 s k) e m) else ret (State f Sskip k e m)
+        | Kreturn k =>
+            do v' <- sem_cast v ty f.(fn_return);
+            do m' <- Mem.free_list m (blocks_of_env e);
+            ret (Returnstate v' (call_cont k) m')
+        | Kswitch1 sl k =>
+            match v with
+            | Vint n => ret (State f (seq_of_labeled_statement (select_switch n sl)) (Kswitch2 k) e m)
+            | _ => nil
+            end
+        | _ => nil
+        end
+
+      | None =>
+          match step_expr e RV a m with
+          | None => nil
+          | Some ll => map (expr_final_state f k e) ll
+          end
+      end
+
+  | State f (Sdo x) k e m => ret(ExprState f x (Kdo k) e m)
+
+  | State f (Ssequence s1 s2) k e m => ret(State f s1 (Kseq s2 k) e m)
+  | State f Sskip (Kseq s k) e m => ret (State f s k e m)
+  | State f Scontinue (Kseq s k) e m => ret (State f Scontinue k e m)
+  | State f Sbreak (Kseq s k) e m => ret (State f Sbreak k e m)
+
+  | State f (Sifthenelse a s1 s2) k e m => ret (ExprState f a (Kifthenelse s1 s2 k) e m)
+
+  | State f (Swhile x s) k e m => ret (ExprState f x (Kwhile1 x s k) e m)
+  | State f (Sskip|Scontinue) (Kwhile2 x s k) e m => ret (State f (Swhile x s) k e m)
+  | State f Sbreak (Kwhile2 x s k) e m => ret (State f Sskip k e m)
+
+  | State f (Sdowhile a s) k e m => ret (State f s (Kdowhile1 a s k) e m)
+  | State f (Sskip|Scontinue) (Kdowhile1 x s k) e m => ret (ExprState f x (Kdowhile2 x s k) e m)
+  | State f Sbreak (Kdowhile1 x s k) e m => ret (State f Sskip k e m)
+
+  | State f (Sfor a1 a2 a3 s) k e m =>
+      if is_skip a1
+      then ret (ExprState f a2 (Kfor2 a2 a3 s k) e m)
+      else ret (State f a1 (Kseq (Sfor Sskip a2 a3 s) k) e m)
+  | State f Sskip (Kfor3 a2 a3 s k) e m => ret (State f a3 (Kfor4 a2 a3 s k) e m)
+  | State f Scontinue (Kfor3 a2 a3 s k) e m => ret (State f a3 (Kfor4 a2 a3 s k) e m)
+  | State f Sbreak (Kfor3 a2 a3 s k) e m => ret (State f Sskip k e m)
+  | State f Sskip (Kfor4 a2 a3 s k) e m => ret (State f (Sfor Sskip a2 a3 s) k e m)
+
+  | State f (Sreturn None) k e m =>
+      do m' <- Mem.free_list m (blocks_of_env e);
+      ret (Returnstate Vundef (call_cont k) m')
+  | State f (Sreturn (Some x)) k e m => ret (ExprState f x (Kreturn k) e m)
+  | State f Sskip ((Kstop | Kcall _ _ _ _ _) as k) e m => 
+     check (type_eq f.(fn_return) Tvoid);
+     do m' <- Mem.free_list m (blocks_of_env e);
+     ret (Returnstate Vundef k m')
+
+  | State f (Sswitch x sl) k e m => ret (ExprState f x (Kswitch1 sl k) e m)
+  | State f (Sskip|Sbreak) (Kswitch2 k) e m => ret (State f Sskip k e m)
+  | State f Scontinue (Kswitch2 k) e m => ret (State f Scontinue k e m)
+
+  | State f (Slabel lbl s) k e m => ret (State f s k e m)
+  | State f (Sgoto lbl) k e m =>
+      match find_label lbl f.(fn_body) (call_cont k) with
+      | Some(s', k') => ret (State f s' k' e m)
+      | None => nil
+      end
+
+  | Callstate (Internal f) vargs k m =>
+      check (list_norepet_dec ident_eq (var_names (fn_params f) ++ var_names (fn_vars f)));
+      let (e,m1) := do_alloc_variables empty_env m (f.(fn_params) ++ f.(fn_vars)) in
+      do m2 <- sem_bind_parameters e m1 f.(fn_params) vargs;
+      ret (State f f.(fn_body) k e m2)
+  | Callstate (External ef _ _) vargs k m =>
+      match do_external _ _ ge ef w vargs m with
+      | None => nil
+      | Some(w',t,v,m') => (t, Returnstate v k m') :: nil
+      end
+
+  | Returnstate v (Kcall f e C ty k) m => ret (ExprState f (C (Eval v ty)) k e m)
+
+  | _ => nil
+  end.
+
+(*
+Definition at_external (S: state): option (external_function * list val * mem) :=
+  match S with
+  | Callstate (External ef _ _) vargs k m => Some (ef, vargs, m)
+  | _ => None
+  end.
+
+Definition after_external (S: state) (v: val) (m: mem): option state :=
+  match S with
+  | Callstate _ _ k _ => Some (Returnstate v k m)
+  | _ => None
+  end.
+*)
+
+Ltac myinv :=
+  match goal with
+  | [ |- In _ nil -> _ ] => intro X; elim X
+  | [ |- In _ (ret _) -> _ ] => 
+        intro X; elim X; clear X;
+        [intro EQ; unfold ret in EQ; inv EQ; myinv | myinv]
+  | [ |- In _ (_ :: nil) -> _ ] => 
+        intro X; elim X; clear X; [intro EQ; inv EQ; myinv | myinv]
+  | [ |- In _ (match ?x with Some _ => _ | None => _ end) -> _ ] => destruct x as []_eqn; myinv
+  | [ |- In _ (match ?x with false => _ | true => _ end) -> _ ] => destruct x as []_eqn; myinv
+  | [ |- In _ (match ?x with left _ => _ | right _ => _ end) -> _ ] => destruct x; myinv
+  | _ => idtac
+  end.
+
+Hint Extern 3 => exact I.
+
+Lemma do_step_sound:
+  forall w S t S', In (t, S') (do_step w S) -> Csem.step ge S t S'.
+Proof with try (right; econstructor; eauto; fail).
+  intros until S'. destruct S; simpl.
+(* State *)
+  destruct s; myinv...
+  (* skip *)
+  destruct k; myinv...
+  (* break *)
+  destruct k; myinv...
+  (* continue *)
+  destruct k; myinv...
+  (* goto *)
+  destruct p as [s' k']. myinv...
+(* ExprState *)
+  destruct (is_val r) as [[v ty]|]_eqn.
+  (* expression is a value *)
+  rewrite (is_val_inv _ _ _ Heqo).
+  destruct k; myinv...
+  destruct v; myinv...
+  (* expression reduces *)
+  destruct (step_expr e RV r m) as [ll|]_eqn; try contradiction. intros.
+  exploit list_in_map_inv; eauto. intros [[C rd] [A B]].
+  generalize (step_expr_sound e r RV m). unfold reducts_ok. rewrite Heqr0. 
+  destruct ll; try contradiction. intros SOUND. 
+  exploit SOUND; eauto. intros [CTX [a [EQ RD]]]. subst r. 
+  unfold expr_final_state in A. simpl in A. left.
+  destruct rd; inv A; simpl in RD. 
+  apply step_lred. auto. apply step_expr_not_stuck; congruence. auto. 
+  apply step_rred. auto. apply step_expr_not_stuck; congruence. auto.
+  destruct RD; subst m'. apply Csem.step_call. auto.  apply step_expr_not_stuck; congruence. auto.
+(* callstate *)
+  destruct fd; myinv.
+  (* internal *)
+  destruct (do_alloc_variables empty_env m (fn_params f ++ fn_vars f)) as [e m1]_eqn.
+  myinv. right; apply step_internal_function with m1. auto. 
+  change e with (fst (e,m1)). change m1 with (snd (e,m1)) at 2. rewrite <- Heqp. 
+  apply do_alloc_variables_sound. apply sem_bind_parameters_sound; auto.
+  (* external *)
+  destruct p as [[[w' tr] v] m']. myinv. right; constructor. 
+  eapply do_ef_external_sound; eauto.
+(* returnstate *)
+  destruct k; myinv...
+Qed.
+
+Remark estep_not_val:
+  forall f a k e m t S, estep ge (ExprState f a k e m) t S -> is_val a = None.
+Proof.
+  intros. 
+  assert (forall b from to C, context from to C -> (C = fun x => x) \/ is_val (C b) = None).
+    induction 1; simpl; auto. 
+  inv H. 
+  destruct (H0 a0 _ _ _ H10). subst. inv H8; auto. auto.
+  destruct (H0 a0 _ _ _ H10). subst. inv H8; auto. auto.
+  destruct (H0 a0 _ _ _ H10). subst. inv H8; auto. auto.
+Qed.
+
+Lemma do_step_complete:
+  forall w S t S' w', possible_trace w t w' -> Csem.step ge S t S' -> In (t, S') (do_step w S).
+Proof with (unfold ret; auto with coqlib).
+  intros until w'; intro PT; intros. 
+  destruct H. 
+  (* Expression step *)
+  inversion H; subst; exploit estep_not_val; eauto; intro NOTVAL.
+(* lred *)
+  unfold do_step; rewrite NOTVAL.
+  destruct (step_expr e RV (C a) m) as [ll|]_eqn.
+  change (E0, ExprState f (C a') k e m') with (expr_final_state f k e (C, Lred a' m')).
+  apply in_map.
+  generalize (step_expr_context e _ _ _ H2 a m). unfold reducts_incl.
+  rewrite Heqr. destruct (step_expr e LV a m) as [ll'|]_eqn; try tauto.
+  intro. replace C with (fun x => C x). apply H3. 
+  rewrite (lred_topred _ _ _ _ _ H0) in Heqr0. inv Heqr0. auto with coqlib.
+  apply extensionality; auto.
+  exploit not_stuck_step_expr; eauto.
+(* rred *)
+  unfold do_step; rewrite NOTVAL.
+  destruct (step_expr e RV (C a) m) as [ll|]_eqn.
+  change (E0, ExprState f (C a') k e m') with (expr_final_state f k e (C, Rred a' m')).
+  apply in_map.
+  generalize (step_expr_context e _ _ _ H2 a m). unfold reducts_incl.
+  rewrite Heqr. destruct (step_expr e RV a m) as [ll'|]_eqn; try tauto.
+  intro. replace C with (fun x => C x). apply H3. 
+  rewrite (rred_topred _ _ _ _ _ H0) in Heqr0. inv Heqr0. auto with coqlib.
+  apply extensionality; auto.
+  exploit not_stuck_step_expr; eauto.
+(* callred *)
+  unfold do_step; rewrite NOTVAL.
+  destruct (step_expr e RV (C a) m) as [ll|]_eqn.
+  change (E0, Callstate fd vargs (Kcall f e C ty k) m) with (expr_final_state f k e (C, Callred fd vargs ty m)).
+  apply in_map.
+  generalize (step_expr_context e _ _ _ H2 a m). unfold reducts_incl.
+  rewrite Heqr. destruct (step_expr e RV a m) as [ll'|]_eqn; try tauto.
+  intro. replace C with (fun x => C x). apply H3. 
+  rewrite (callred_topred _ _ _ _ _ _ H0) in Heqr0. inv Heqr0. auto with coqlib.
+  apply extensionality; auto.
+  exploit not_stuck_step_expr; eauto.
+
+  (* Statement step *)
+  inv H; simpl...
+  rewrite H0...
+  rewrite H0...
+  rewrite H0...
+  destruct H0; subst s0...
+  destruct H0; subst s0...
+  rewrite H0...
+  rewrite H0...
+  rewrite pred_dec_false...
+  rewrite pred_dec_true...
+  rewrite H0...
+  rewrite H0...
+  destruct H0; subst x...
+  rewrite H0...
+  rewrite H0; rewrite H1...
+  rewrite pred_dec_true; auto. rewrite H2. red in H0. destruct k; try contradiction...
+  destruct H0; subst x...
+  rewrite H0...
+
+  (* Call step *)
+  rewrite pred_dec_true; auto. rewrite (do_alloc_variables_complete _ _ _ _ _ H1).
+  rewrite (sem_bind_parameters_complete _ _ _ _ _ H2)...
+  exploit do_ef_external_complete; eauto. intro EQ; rewrite EQ. auto with coqlib.
+Qed.
+
+End EXEC.
+
+Local Open Scope option_monad_scope.
+
+Definition do_initial_state (p: program): option (genv * state) :=
+  let ge := Genv.globalenv p in
+  do m0 <- Genv.init_mem p;
+  do b <- Genv.find_symbol ge p.(prog_main);
+  do f <- Genv.find_funct_ptr ge b;
+  check (type_eq (type_of_fundef f) (Tfunction Tnil (Tint I32 Signed)));
+  Some (ge, Callstate f nil Kstop m0).
+
+Definition at_final_state (S: state): option int :=
+  match S with
+  | Returnstate (Vint r) Kstop m => Some r
+  | _ => None
+  end.
